src/Parsers/BooleanRecognizerCorrect.v
@@ -1,6 +1,6 @@
 (** * Definition of a boolean-returning CFG parser-recognizer *)
 Require Import Coq.Lists.List Coq.Program.Program Coq.Program.Wf Coq.Arith.Wf_nat Coq.Arith.Compare_dec Coq.Classes.RelationClasses Coq.Strings.String.
-Require Import Parsers.ContextFreeGrammar Parsers.BooleanRecognizer Parsers.MinimalParse.
+Require Import Parsers.BaseTypes Parsers.ContextFreeGrammar Parsers.BooleanRecognizer Parsers.MinimalParse.
 Require Import Parsers.MinimalParseOfParse.
 Require Import Parsers.ContextFreeGrammarProperties Parsers.WellFoundedParse.
 Require Import Common Common.Wf.
@@ -19,59 +19,44 @@ Local Open Scope string_like_scope.
 Section sound.
   Section general.
     Context CharType (String : string_like CharType) (G : grammar CharType).
-    Context (names_listT : Type)
-            (initial_names_data : names_listT)
-            (is_valid_name : names_listT -> string -> bool)
-            (remove_name : names_listT -> string -> names_listT)
-            (names_listT_R : names_listT -> names_listT -> Prop)
-            (remove_name_dec : forall ls name, is_valid_name ls name = true
-                                               -> names_listT_R (remove_name ls name) ls)
-            (ntl_wf : well_founded names_listT_R)
-            (split_stateT : String -> Type)
-            (remove_name_1
+    Context `{data : @boolean_parser_dataT CharType String}.
+    Context (remove_nonterminal_1
              : forall ls ps ps',
-                 is_valid_name (remove_name ls ps) ps' = true
-                 -> is_valid_name ls ps' = true)
-            (remove_name_2
+                 is_valid_nonterminal (remove_nonterminal ls ps) ps' = true
+                 -> is_valid_nonterminal ls ps' = true)
+            (remove_nonterminal_2
              : forall ls ps ps',
-                 is_valid_name (remove_name ls ps) ps' = false
-                 <-> is_valid_name ls ps' = false \/ ps = ps')
-            (split_string_for_production
-             : forall (str0 : StringWithSplitState String split_stateT) (prod : production CharType), list (StringWithSplitState String split_stateT * StringWithSplitState String split_stateT))
-            (split_string_for_production_correct
-             : forall (str0 : StringWithSplitState String split_stateT) prod,
-                 List.Forall (fun s1s2 : StringWithSplitState String split_stateT * StringWithSplitState String split_stateT
-                              => fst s1s2 ++ snd s1s2 =s str0)
-                             (split_string_for_production str0 prod)).
+                 is_valid_nonterminal (remove_nonterminal ls ps) ps' = false
+                 <-> is_valid_nonterminal ls ps' = false \/ ps = ps').
 
     Let P : string -> Prop
-      := fun p => is_valid_name initial_names_data p = true.
+      := fun p => is_valid_nonterminal initial_nonterminals_data p = true.
 
     Section parts.
       Local Hint Constructors parse_of_item parse_of parse_of_production.
 
       (*Let H_subT valid
-        := sub_productions_listT is_valid_name valid initial_names_data.*)
+        := sub_productions_listT is_valid_nonterminal valid initial_nonterminals_data.*)
 
       Section item.
         Context (str : StringWithSplitState String split_stateT)
-                (str_matches_name : string -> bool).
+                (str_matches_nonterminal : string -> bool).
 
-        Definition str_matches_name_soundT
-          := forall name, str_matches_name name = true
-                          -> parse_of_item _ G str (NonTerminal _ name).
+        Definition str_matches_nonterminal_soundT
+          := forall nonterminal, str_matches_nonterminal nonterminal = true
+                          -> parse_of_item _ G str (NonTerminal _ nonterminal).
 
-        Definition str_matches_name_completeT P str0
-          := forall (valid : names_listT) name (H_sub : P str0 valid name),
-               minimal_parse_of_item _ G initial_names_data is_valid_name remove_name str0 valid str (NonTerminal _ name)
-               -> str_matches_name name = true.
+        Definition str_matches_nonterminal_completeT P str0
+          := forall (valid : nonterminals_listT) nonterminal (H_sub : P str0 valid nonterminal),
+               minimal_parse_of_item _ G initial_nonterminals_data is_valid_nonterminal remove_nonterminal str0 valid str (NonTerminal _ nonterminal)
+               -> str_matches_nonterminal nonterminal = true.
 
         Lemma parse_item_sound
-              (str_matches_name_sound : str_matches_name_soundT)
+              (str_matches_nonterminal_sound : str_matches_nonterminal_soundT)
               (it : item CharType)
-        : parse_item str str_matches_name it = true -> parse_of_item _ G str it.
+        : parse_item str_matches_nonterminal str it = true -> parse_of_item _ G str it.
         Proof.
-          unfold parse_item, str_matches_name_soundT in *.
+          unfold parse_item, str_matches_nonterminal_soundT in *.
           repeat match goal with
                    | _ => intro
                    | [ H : context[match ?E with _ => _ end] |- _ ] => atomic E; destruct E
@@ -87,15 +72,15 @@ Section sound.
         Lemma parse_item_complete
               str0
               valid Pv
-              (str_matches_name_complete : str_matches_name_completeT Pv str0)
+              (str_matches_nonterminal_complete : str_matches_nonterminal_completeT Pv str0)
               (it : item CharType)
-              (Hinit : forall name,
-                         minimal_parse_of_name String G initial_names_data is_valid_name remove_name str0 valid str name
-                         -> Pv str0 valid name)
-        : minimal_parse_of_item _ G initial_names_data is_valid_name remove_name str0 valid str it
-          -> parse_item str str_matches_name it = true.
+              (Hinit : forall nonterminal,
+                         minimal_parse_of_name String G initial_nonterminals_data is_valid_nonterminal remove_nonterminal str0 valid str nonterminal
+                         -> Pv str0 valid nonterminal)
+        : minimal_parse_of_item _ G initial_nonterminals_data is_valid_nonterminal remove_nonterminal str0 valid str it
+          -> parse_item str_matches_nonterminal str it = true.
         Proof.
-          unfold parse_item, str_matches_name_completeT in *.
+          unfold parse_item, str_matches_nonterminal_completeT in *.
           repeat
             repeat
             match goal with
@@ -110,11 +95,11 @@ Section sound.
               | [ |- _ = true ] => apply bool_eq_correct
               | [ H : context[?E] |- context[match ?E with _ => _ end] ] => destruct E
               | [ H : minimal_parse_of _ _ _ _ _ _ _ [] |- _ ] => solve [ inversion H ]
-              | [ |- str_matches_name _ = true ]
-                => eapply str_matches_name_complete; [..| eassumption ]
+              | [ |- str_matches_nonterminal _ = true ]
+                => eapply str_matches_nonterminal_complete; [..| eassumption ]
               | [ H : minimal_parse_of_item _ _ _ _ _ _ _ _ (Terminal _) |- _ ] => inversion_clear H
               | [ H : minimal_parse_of_item _ _ _ _ _ _ _ _ (NonTerminal _ _) |- _ ] => inversion_clear H
-              | [ H : forall name, _ -> Pv _ _ name |- Pv _ _ _ ] => eapply H
+              | [ H : forall nonterminal, _ -> Pv _ _ nonterminal |- Pv _ _ _ ] => eapply H
           end.
         Qed.
       End item.
@@ -122,11 +107,11 @@ Section sound.
       Section item_ext.
         Lemma parse_item_ext
               (str : StringWithSplitState String split_stateT)
-              (str_matches_name1 str_matches_name2 : string -> bool)
+              (str_matches_nonterminal1 str_matches_nonterminal2 : string -> bool)
               (it : item CharType)
-              (ext : forall x, str_matches_name1 x = str_matches_name2 x)
-        : parse_item str str_matches_name1 it
-          = parse_item str str_matches_name2 it.
+              (ext : forall x, str_matches_nonterminal1 x = str_matches_nonterminal2 x)
+        : parse_item str_matches_nonterminal1 str it
+          = parse_item str_matches_nonterminal2 str it.
         Proof.
           unfold parse_item.
           destruct it; auto;
@@ -138,32 +123,24 @@ Section sound.
       End item_ext.
 
       Section production.
-        Context (str0 : StringWithSplitState String split_stateT)
-                (parse_name : forall (str : StringWithSplitState String split_stateT),
+        Context (str0 : String)
+                (parse_nonterminal : forall (str : StringWithSplitState String split_stateT),
                                 str ≤s str0
                                 -> string
                                 -> bool).
 
-        Definition parse_name_soundT
-          := forall str pf name,
-               @parse_name str pf name = true
-               -> parse_of_item _ G str (NonTerminal _ name).
+        Definition parse_nonterminal_soundT
+          := forall str pf nonterminal,
+               @parse_nonterminal str pf nonterminal = true
+               -> parse_of_item _ G str (NonTerminal _ nonterminal).
 
-        Definition parse_name_completeT P
-          := forall valid (str : StringWithSplitState String split_stateT) pf name (H_sub : P str0 valid name),
-               minimal_parse_of_name _ G initial_names_data is_valid_name remove_name str0 valid str name
-               -> @parse_name str pf name = true.
-
-        Definition split_correctT
-                   (str1 : StringWithSplitState String split_stateT)
-                   (split : StringWithSplitState String split_stateT * StringWithSplitState String split_stateT)
-          := fst split ++ snd split =s str1.
-
-        Definition split_list_correctT str1 (split_list : list (StringWithSplitState String split_stateT * StringWithSplitState String split_stateT))
-          := List.Forall (@split_correctT str1) split_list.
+        Definition parse_nonterminal_completeT P
+          := forall valid (str : StringWithSplitState String split_stateT) pf nonterminal (H_sub : P str0 valid nonterminal),
+               minimal_parse_of_name _ G initial_nonterminals_data is_valid_nonterminal remove_nonterminal str0 valid str nonterminal
+               -> @parse_nonterminal str pf nonterminal = true.
 
         Definition split_list_completeT
-                   valid1 valid2
+                   valid
                    (str : StringWithSplitState String split_stateT) (pf : str ≤s str0)
                    (split_list : list (StringWithSplitState String split_stateT * StringWithSplitState String split_stateT))
                    (prod : production CharType)
@@ -171,22 +148,22 @@ Section sound.
                | nil => True
                | it::its => ({ s1s2 : String * String
                                       & (fst s1s2 ++ snd s1s2 =s str)
-                                        * (minimal_parse_of_item _ G initial_names_data is_valid_name remove_name str0 valid1 (fst s1s2) it)
-                                        * (minimal_parse_of_production _ G initial_names_data is_valid_name remove_name str0 valid2 (snd s1s2) its) }%type)
+                                        * (minimal_parse_of_item _ G initial_nonterminals_data is_valid_nonterminal remove_nonterminal str0 valid (fst s1s2) it)
+                                        * (minimal_parse_of_production _ G initial_nonterminals_data is_valid_nonterminal remove_nonterminal str0 valid (snd s1s2) its) }%type)
                             -> ({ s1s2 : StringWithSplitState String split_stateT * StringWithSplitState String split_stateT
                                          & (In s1s2 split_list)
-                                           * (minimal_parse_of_item _ G initial_names_data is_valid_name remove_name str0 valid1 (fst s1s2) it)
-                                           * (minimal_parse_of_production _ G initial_names_data is_valid_name remove_name str0 valid2 (snd s1s2) its) }%type)
+                                           * (minimal_parse_of_item _ G initial_nonterminals_data is_valid_nonterminal remove_nonterminal str0 valid (fst s1s2) it)
+                                           * (minimal_parse_of_production _ G initial_nonterminals_data is_valid_nonterminal remove_nonterminal str0 valid (snd s1s2) its) }%type)
              end.
 
         Lemma parse_production_sound
-                 (parse_name_sound : parse_name_soundT)
+                 (parse_nonterminal_sound : parse_nonterminal_soundT)
                  (str : StringWithSplitState String split_stateT) (pf : str ≤s str0)
                  (prod : production CharType)
-        : parse_production split_string_for_production split_string_for_production_correct str0 parse_name str pf prod = true
+        : parse_production parse_nonterminal str pf prod = true
           -> parse_of_production _ G str prod.
         Proof.
-          change (forall str0 prod, split_list_correctT str0 (split_string_for_production str0 prod)) in split_string_for_production_correct.
+          (*change (forall str0 it its, split_list_correctT str0 (split_string_for_production it its)) in split_string_for_production_correct.*)
           revert str pf; induction prod;
           repeat match goal with
                    | _ => intro
@@ -198,6 +175,7 @@ Section sound.
                    | [ H : (_ && _)%bool = true |- _ ] => apply Bool.andb_true_iff in H
                    | _ => progress destruct_head sumbool
                    | _ => progress destruct_head and
+                   | _ => progress destruct_head prod
                    | _ => progress destruct_head sig
                    | _ => progress destruct_head @StringWithSplitState
                    | _ => progress simpl in *
@@ -208,27 +186,31 @@ Section sound.
                         pose proof H as H';
                           apply bool_eq_correct in H';
                           progress subst
+                   | [ |- parse_of_production _ _ (_ ++ Empty _) [?it] ]
+                     => constructor
+                   | [ |- parse_of_item _ _ ?s _ ]
+                     => eapply parse_item_sound with (str := {| string_val := s |});
+                       hnf in *; solve [ eauto with nocore ]
                  end.
           { constructor;
             solve [ eapply IHprod; eassumption
                   | eapply parse_item_sound; try eassumption;
-                    hnf in parse_name_sound |- *;
-                    apply parse_name_sound ]. }
+                    hnf in parse_nonterminal_sound |- *;
+                    apply parse_nonterminal_sound ]. }
         Defined.
 
         Lemma parse_production_complete
               valid Pv
-              (parse_name_complete : parse_name_completeT Pv)
-              (split_string_for_production_complete : forall valid1 valid2 str pf prod, @split_list_completeT valid1 valid2 str pf (split_string_for_production str prod) prod)
-              (Hinit : forall str (pf : str ≤s str0) name,
-                         minimal_parse_of_name String G initial_names_data is_valid_name remove_name str0 valid str name
-                         -> Pv str0 valid name)
+              (parse_nonterminal_complete : parse_nonterminal_completeT Pv)
+              (split_string_for_production_complete : forall valid str pf it its, @split_list_completeT valid str pf (split_string_for_production it its str) (it::its))
+              (Hinit : forall str (pf : str ≤s str0) nonterminal,
+                         minimal_parse_of_name String G initial_nonterminals_data is_valid_nonterminal remove_nonterminal str0 valid str nonterminal
+                         -> Pv str0 valid nonterminal)
               (str : StringWithSplitState String split_stateT) (pf : str ≤s str0)
               (prod : production CharType)
-        : minimal_parse_of_production _ G initial_names_data is_valid_name remove_name str0 valid str prod
-          -> parse_production split_string_for_production split_string_for_production_correct str0 parse_name str pf prod = true.
+        : minimal_parse_of_production _ G initial_nonterminals_data is_valid_nonterminal remove_nonterminal str0 valid str prod
+          -> parse_production parse_nonterminal str pf prod = true.
         Proof.
-          change (forall str0 prod, split_list_correctT str0 (split_string_for_production str0 prod)) in split_string_for_production_correct.
           revert valid str Hinit pf; induction prod;
           repeat match goal with
                    | _ => intro
@@ -255,29 +237,28 @@ Section sound.
                           apply bool_eq_correct in H';
                           progress subst
                    | [ H : minimal_parse_of_production _ _ _ _ _ _ _ _ (_::_) |- _ ] => inversion H; clear H; subst
-                   | [ H : ?s ≤s _ |- context[split_string_for_production_correct {| string_val := ?s ; state_val := ?st |} ?p] ]
-                     => specialize (fun a b p0 v1 p1 v2 p2
-                                    => @split_string_for_production_complete v1 v2 {| string_val := s ; state_val := st |} H p (existT _ (a, b) (p0, p1, p2)))
+                   | [ H : ?s ≤s _ |- context[split_string_for_production_correct ?it ?p {| string_val := ?s ; state_val := ?st |}] ]
+                     => specialize (fun a b p0 v p1 p2
+                                    => @split_string_for_production_complete v {| string_val := s ; state_val := st |} H it p (existT _ (a, b) (p0, p1, p2)))
                    | [ H : forall a b, is_true (string_val a ++ string_val b =s _ ++ _) -> _ |- _ ]
                      => specialize (fun st0 st1 => H {| state_val := st0 |} {| state_val := st1 |} (proj2 (@bool_eq_correct _ _ _ _) eq_refl))
                    | [ H : forall a b, is_true (a ++ b =s _ ++ _) -> _ |- _ ]
                      => specialize (H _ _ (proj2 (@bool_eq_correct _ _ _ _) eq_refl))
                    | [ H : ?a -> ?b, H' : ?a |- _ ] => specialize (H H')
-                   | [ H : forall v : names_listT, @?a v -> @?b v |- _ ]
-                     => pose proof (H valid); pose proof (H initial_names_data); clear H
+                   | [ H : forall v : nonterminals_listT, @?a v -> @?b v |- _ ]
+                     => pose proof (H valid); pose proof (H initial_nonterminals_data); clear H
                    | [ |- fold_right orb false (map _ _) = true ] => apply fold_right_orb_map_sig2
                    | [ H : minimal_parse_of_item _ _ _ _ _ _ _ _ _ |- _ ] => inversion H; clear H; subst
                    | [ |- (_ =s _) = true ] => apply bool_eq_correct
                  end;
-          match goal with
-            | [ H : In (?s1, ?s2) (split_string_for_production {| string_val := ?str ; state_val := ?st |} ?prod)
+          (lazymatch goal with
+            | [ H : In (?s1, ?s2) (split_string_for_production ?it ?prod {| string_val := ?str ; state_val := ?st |})
                 |- { x : { s1s2 : _ | (?f (fst s1s2) ++ ?f (snd s1s2) =s ?str) = true } | _ } ]
               => let H' := fresh in
-                 pose proof (proj1 (@Forall_forall _ _ _) (@split_string_for_production_correct {| string_val := str ; state_val := st |} prod) _ H) as H';
-                   unfold split_correctT in H';
+                 pose proof (proj1 (@Forall_forall _ _ _) (split_string_for_production_correct it prod {| string_val := str ; state_val := st |}) _ H) as H';
                    refine (exist _ (exist _ (s1, s2) _) _);
                    simpl in *
-          end;
+          end);
           repeat match goal with
                    | _ => split
                    | [ |- (_ && _)%bool = true ] => apply Bool.andb_true_iff
@@ -285,7 +266,7 @@ Section sound.
                    | [ |- In _ (combine_sig _) ] => apply In_combine_sig
                    | [ IHprod : _ |- _ ] => eapply IHprod; eassumption
                  end;
-          eapply parse_name_complete; [..| eassumption ]; simpl;
+          eapply parse_nonterminal_complete; [..| eassumption ]; simpl;
           repeat match goal with
                    | _ => eassumption
                    | _ => reflexivity
@@ -302,16 +283,16 @@ Section sound.
 
       Section production_ext.
         Lemma parse_production_ext
-              (str0 : StringWithSplitState String split_stateT)
-              (parse_name1 parse_name2 : forall (str : StringWithSplitState String split_stateT),
+              (str0 : String)
+              (parse_nonterminal1 parse_nonterminal2 : forall (str : StringWithSplitState String split_stateT),
                                            str ≤s str0
                                            -> string
                                            -> bool)
               (str : StringWithSplitState String split_stateT) (pf : str ≤s str0) (prod : production CharType)
-              (ext : forall str' pf' name', parse_name1 str' pf' name'
-                                            = parse_name2 str' pf' name')
-        : parse_production split_string_for_production split_string_for_production_correct str0 parse_name1 str pf prod
-          = parse_production split_string_for_production split_string_for_production_correct str0 parse_name2 str pf prod.
+              (ext : forall str' pf' nonterminal', parse_nonterminal1 str' pf' nonterminal'
+                                            = parse_nonterminal2 str' pf' nonterminal')
+        : parse_production parse_nonterminal1 str pf prod
+          = parse_production parse_nonterminal2 str pf prod.
         Proof.
           revert str pf.
           induction prod as [|? ? IHprod]; simpl; intros; try reflexivity; [].
@@ -323,8 +304,8 @@ Section sound.
       End production_ext.
 
       Section productions.
-        Context (str0 : StringWithSplitState String split_stateT)
-                (parse_name : forall (str : StringWithSplitState String split_stateT),
+        Context (str0 : String)
+                (parse_nonterminal : forall (str : StringWithSplitState String split_stateT),
                                 str ≤s str0
                                 -> string
                                 -> bool).
@@ -348,19 +329,18 @@ Section sound.
                    | [ H : parse_of _ _ _ (_::_) |- _ ] => inversion H; clear H; subst
                    | [ H : minimal_parse_of _ _ _ _ _ _ _ _ nil |- _ ] => solve [ inversion H ]
                    | [ H : minimal_parse_of _ _ _ _ _ _ _ _ (_::_) |- _ ] => inversion H; clear H; subst
-                   | [ H : parse_production _ _ _ _ _ _ _ = true |- _ ] => apply parse_production_sound in H; try eassumption; []
+                   | [ H : parse_production _ _ _ _ = true |- _ ] => apply parse_production_sound with (str := {| string_val := _ |}) in H; try eassumption; []
                    | _ => left; eapply parse_production_complete; eassumption
                    | _ => solve [ eauto ]
                  end.
 
         Lemma parse_productions_sound
-                 (parse_name_sound : parse_name_soundT str0 parse_name)
+                 (parse_nonterminal_sound : parse_nonterminal_soundT parse_nonterminal)
                  (str : StringWithSplitState String split_stateT) (pf : str ≤s str0)
                  (prods : productions CharType)
-        : parse_productions split_string_for_production split_string_for_production_correct str0 parse_name str pf prods = true
+        : parse_productions parse_nonterminal str pf prods = true
           -> parse_of _ G str prods.
         Proof.
-          change (forall str0 prod, split_list_correctT str0 (split_string_for_production str0 prod)) in split_string_for_production_correct.
           destruct str as [str st]; simpl in *.
           revert str pf st; induction prods; simpl.
           { unfold parse_productions; simpl; intros ??? H; exfalso; clear -H.
@@ -371,17 +351,16 @@ Section sound.
 
         Lemma parse_productions_complete
               valid Pv
-              (parse_name_complete : parse_name_completeT str0 parse_name Pv)
-              (split_string_for_production_complete : forall valid1 valid2 str pf prod, @split_list_completeT str0 valid1 valid2 str pf (split_string_for_production str prod) prod)
-              (Hinit : forall str (pf : str ≤s str0) name,
-                         minimal_parse_of_name String G initial_names_data is_valid_name remove_name str0 valid str name
-                         -> Pv str0 valid name)
+              (parse_nonterminal_complete : parse_nonterminal_completeT parse_nonterminal Pv)
+              (split_string_for_production_complete : forall valid str pf it its, @split_list_completeT str0 valid str pf (split_string_for_production it its str) (it::its))
+              (Hinit : forall str (pf : str ≤s str0) nonterminal,
+                         minimal_parse_of_name String G initial_nonterminals_data is_valid_nonterminal remove_nonterminal str0 valid str nonterminal
+                         -> Pv str0 valid nonterminal)
               (str : StringWithSplitState String split_stateT) (pf : str ≤s str0)
               (prods : productions CharType)
-        : minimal_parse_of _ G initial_names_data is_valid_name remove_name str0 valid str prods
-          -> parse_productions split_string_for_production split_string_for_production_correct str0 parse_name str pf prods = true.
+        : minimal_parse_of _ G initial_nonterminals_data is_valid_nonterminal remove_nonterminal str0 valid str prods
+          -> parse_productions parse_nonterminal str pf prods = true.
         Proof.
-          change (forall str0 prod, split_list_correctT str0 (split_string_for_production str0 prod)) in split_string_for_production_correct.
           destruct str as [str st]; simpl in *.
           revert str pf st; induction prods; simpl.
           { unfold parse_productions; simpl; intros ??? H; exfalso; clear -H.
@@ -393,16 +372,16 @@ Section sound.
 
       Section productions_ext.
         Lemma parse_productions_ext
-              (str0 : StringWithSplitState String split_stateT)
-              (parse_name1 parse_name2 : forall (str : StringWithSplitState String split_stateT),
+              (str0 : String)
+              (parse_nonterminal1 parse_nonterminal2 : forall (str : StringWithSplitState String split_stateT),
                                            str ≤s str0
                                            -> string
                                            -> bool)
               (str : StringWithSplitState String split_stateT) (pf : str ≤s str0) (prods : productions CharType)
-              (ext : forall str' pf' name', parse_name1 str' pf' name'
-                                            = parse_name2 str' pf' name')
-        : parse_productions split_string_for_production split_string_for_production_correct str0 parse_name1 str pf prods
-          = parse_productions split_string_for_production split_string_for_production_correct str0 parse_name2 str pf prods.
+              (ext : forall str' pf' nonterminal', parse_nonterminal1 str' pf' nonterminal'
+                                            = parse_nonterminal2 str' pf' nonterminal')
+        : parse_productions parse_nonterminal1 str pf prods
+          = parse_productions parse_nonterminal2 str pf prods.
         Proof.
           revert str pf.
           induction prods as [|? ? IHprod]; simpl; intros; try reflexivity; [].
@@ -412,62 +391,58 @@ Section sound.
         Qed.
       End productions_ext.
 
-      Section names.
+      Section nonterminals.
         Section step.
-          Context (str0 : StringWithSplitState String split_stateT) (valid : names_listT)
-                  (parse_name
-                   : forall (p : StringWithSplitState String split_stateT * names_listT),
-                       prod_relation (ltof _ (fun s : StringWithSplitState String split_stateT => Length s)) names_listT_R p (str0, valid)
+          Context (str0 : String) (valid : nonterminals_listT)
+                  (parse_nonterminal
+                   : forall (p : String * nonterminals_listT),
+                       prod_relation (ltof _ Length) nonterminals_listT_R p (str0, valid)
                        -> forall str : StringWithSplitState String split_stateT, str ≤s fst p -> string -> bool).
 
-          Lemma parse_name_step_sound
-                (parse_name_sound : forall p pf, parse_name_soundT _ (@parse_name p pf))
-                (str : StringWithSplitState String split_stateT) (pf : str ≤s str0) (name : string)
-          : parse_name_step G initial_names_data is_valid_name remove_name
-                            remove_name_dec split_string_for_production
-                            split_string_for_production_correct parse_name _ pf name
+          Lemma parse_nonterminal_step_sound
+                (parse_nonterminal_sound : forall p pf, parse_nonterminal_soundT (@parse_nonterminal p pf))
+                (str : StringWithSplitState String split_stateT) (pf : str ≤s str0) (nonterminal : string)
+          : parse_nonterminal_step (G := G) parse_nonterminal _ pf nonterminal
             = true
-            -> parse_of_item _ G str (NonTerminal _ name).
+            -> parse_of_item _ G str (NonTerminal _ nonterminal).
           Proof.
-            unfold parse_name_step.
+            unfold parse_nonterminal_step.
             intro H'; constructor; revert H'.
             edestruct lt_dec as [|n].
             { intro H'.
               apply parse_productions_sound in H'; trivial. }
             { edestruct dec; [ | intro H''; exfalso; clear -H'';
                                  abstract discriminate ].
-              apply strle_to_sumbool in pf.
-              destruct pf as [pf|]; subst.
-              { destruct (n pf). }
+              pose proof (strle_to_sumbool _ pf) as pf'.
+              destruct pf' as [pf'|]; subst.
+              { destruct (n pf'). }
               { intro H'.
                 apply parse_productions_sound in H'; trivial;
                 destruct_head @StringWithSplitState; subst; trivial. } }
           Defined.
 
-          Lemma parse_name_step_complete
+          Lemma parse_nonterminal_step_complete
                 Pv
-                (parse_name_complete : forall p pf, parse_name_completeT _ (@parse_name p pf) (Pv p))
-                (split_string_for_production_complete : forall str0 valid1 valid2 str pf prod, @split_list_completeT str0 valid1 valid2 str pf (split_string_for_production str prod) prod)
-                (str : StringWithSplitState String split_stateT) (pf : str ≤s str0) (name : string)
+                (parse_nonterminal_complete : forall p pf, parse_nonterminal_completeT (@parse_nonterminal p pf) (Pv p))
+                (split_string_for_production_complete : forall str0 valid str pf it its, @split_list_completeT str0 valid str pf (split_string_for_production it its str) (it::its))
+                (str : StringWithSplitState String split_stateT) (pf : str ≤s str0) (nonterminal : string)
                 (Hinit : forall str1,
                            str1 ≤s str ->
-                           forall name0,
-                             minimal_parse_of_name String G initial_names_data is_valid_name
-                                                   remove_name str initial_names_data str1 name0 ->
-                             Pv (str, initial_names_data) str initial_names_data name0)
+                           forall nonterminal0,
+                             minimal_parse_of_name String G initial_nonterminals_data is_valid_nonterminal
+                                                   remove_nonterminal str initial_nonterminals_data str1 nonterminal0 ->
+                             Pv (str : String, initial_nonterminals_data) str initial_nonterminals_data nonterminal0)
                 (Hinit' : forall str,
                             str ≤s str0 ->
-                            forall name0 : string,
-                              minimal_parse_of_name String G initial_names_data is_valid_name remove_name
-                                                    str0 (remove_name valid name) str name0 ->
-                              Pv (str0, remove_name valid name) str0 (remove_name valid name) name0)
-          : minimal_parse_of_name _ G initial_names_data is_valid_name remove_name str0 valid str name
-            -> parse_name_step G initial_names_data is_valid_name remove_name
-                            remove_name_dec split_string_for_production
-                            split_string_for_production_correct parse_name _ pf name
+                            forall nonterminal0 : string,
+                              minimal_parse_of_name String G initial_nonterminals_data is_valid_nonterminal remove_nonterminal
+                                                    str0 (remove_nonterminal valid nonterminal) str nonterminal0 ->
+                              Pv (str0, remove_nonterminal valid nonterminal) str0 (remove_nonterminal valid nonterminal) nonterminal0)
+          : minimal_parse_of_name _ G initial_nonterminals_data is_valid_nonterminal remove_nonterminal str0 valid str nonterminal
+            -> parse_nonterminal_step (G := G) parse_nonterminal _ pf nonterminal
             = true.
           Proof.
-            unfold parse_name_step.
+            unfold parse_nonterminal_step.
             edestruct lt_dec as [|n].
             { intros H'.
               inversion H'; clear H'; subst. (* Work around Anomaly: Evar ?425 was not declared. Please report. *)
@@ -487,7 +462,7 @@ Section sound.
                     end. }
                   { let H' := match goal with H : minimal_parse_of _ _ _ _ _ _ _ _ _ |- _ => constr:H end in
                     eapply parse_productions_complete in H'; eauto.
-                    eapply (@parse_name_complete (_, _)). } }
+                    eapply (@parse_nonterminal_complete (_, _)). } }
                 { intro H''; exfalso; clear -n H'' pf'.
                   abstract (
                       inversion_clear H'';
@@ -497,21 +472,17 @@ Section sound.
         End step.
 
         Section step_extensional.
-          Lemma parse_name_step_ext (str0 : StringWithSplitState String split_stateT) (valid : names_listT)
-                (parse_name1 parse_name2: forall (p : StringWithSplitState String split_stateT * names_listT),
-                                            prod_relation (ltof _ (fun s : StringWithSplitState String split_stateT => Length s)) names_listT_R p (str0, valid)
+          Lemma parse_nonterminal_step_ext (str0 : String) (valid : nonterminals_listT)
+                (parse_nonterminal1 parse_nonterminal2: forall (p : String * nonterminals_listT),
+                                            prod_relation (ltof _ Length) nonterminals_listT_R p (str0, valid)
                                             -> forall str : StringWithSplitState String split_stateT, str ≤s fst p -> string -> bool)
-                (str : StringWithSplitState String split_stateT) (pf : str ≤s str0) (name : string)
-                (ext : forall p pf0 str' pf' name', parse_name1 p pf0 str' pf' name'
-                                                    = parse_name2 p pf0 str' pf' name')
-          : parse_name_step G initial_names_data is_valid_name remove_name
-                            remove_name_dec split_string_for_production
-                            split_string_for_production_correct parse_name1 _ pf name
-            = parse_name_step G initial_names_data is_valid_name remove_name
-                              remove_name_dec split_string_for_production
-                              split_string_for_production_correct parse_name2 _ pf name.
+                (str : StringWithSplitState String split_stateT) (pf : str ≤s str0) (nonterminal : string)
+                (ext : forall p pf0 str' pf' nonterminal', parse_nonterminal1 p pf0 str' pf' nonterminal'
+                                                    = parse_nonterminal2 p pf0 str' pf' nonterminal')
+          : parse_nonterminal_step (G := G) parse_nonterminal1 _ pf nonterminal
+            = parse_nonterminal_step (G := G) parse_nonterminal2 _ pf nonterminal.
           Proof.
-            unfold parse_name_step.
+            unfold parse_nonterminal_step.
             edestruct lt_dec.
             { apply parse_productions_ext; auto. }
             { edestruct dec; trivial.
@@ -520,26 +491,23 @@ Section sound.
         End step_extensional.
 
         Section wf.
-          Lemma parse_name_or_abort_sound
-                (p : StringWithSplitState String split_stateT * names_listT) (str : StringWithSplitState String split_stateT)
+          Lemma parse_nonterminal_or_abort_sound
+                (p : String * nonterminals_listT) (str : StringWithSplitState String split_stateT)
                 (pf : str ≤s fst p)
-                (name : string)
-          : parse_name_or_abort G initial_names_data is_valid_name remove_name
-                                remove_name_dec ntl_wf split_string_for_production
-                                split_string_for_production_correct
-                                p _ pf name
+                (nonterminal : string)
+          : parse_nonterminal_or_abort (G := G) p _ pf nonterminal
             = true
-            -> parse_of_item _ G str (NonTerminal _ name).
+            -> parse_of_item _ G str (NonTerminal _ nonterminal).
           Proof.
-            unfold parse_name_or_abort.
-            revert str pf name.
+            unfold parse_nonterminal_or_abort.
+            revert str pf nonterminal.
             let Acca := match goal with |- context[@Fix3 _ _ _ _ _ ?Rwf _ _ ?a _ _ _] => constr:(Rwf a) end in
             induction (Acca) as [? ? IHr];
-              intros str pf name.
+              intros str pf nonterminal.
             rewrite Fix3_eq.
-            { apply parse_name_step_sound; assumption. }
+            { apply parse_nonterminal_step_sound; assumption. }
             { intros.
-              apply parse_name_step_ext.
+              apply parse_nonterminal_step_ext.
               trivial. }
           Defined.
 
@@ -555,84 +523,76 @@ Section sound.
             { exact H. }
           Qed.
 
-          Lemma parse_name_or_abort_complete
-                (split_string_for_production_complete : forall str0 valid1 valid2 str pf prod, @split_list_completeT str0 valid1 valid2 str pf (split_string_for_production str prod) prod)
-                (Pv := fun (p : StringWithSplitState String split_stateT * names_listT)
-                           (str0 : StringWithSplitState String split_stateT) (valid0 : names_listT) (_ : string) =>
-                         sub_names_listT is_valid_name valid0 (snd p)
-                         /\ sub_names_listT is_valid_name (snd p) initial_names_data)
-                (p : StringWithSplitState String split_stateT * names_listT)
-          : @parse_name_completeT
+          Lemma parse_nonterminal_or_abort_complete
+                (split_string_for_production_complete : forall str0 valid str pf it its, @split_list_completeT str0 valid str pf (split_string_for_production it its str) (it::its))
+                (Pv := fun (p : String * nonterminals_listT)
+                           (str0 : String) (valid0 : nonterminals_listT) (_ : string) =>
+                         sub_names_listT is_valid_nonterminal valid0 (snd p)
+                         /\ sub_names_listT is_valid_nonterminal (snd p) initial_nonterminals_data)
+                (p : String * nonterminals_listT)
+          : @parse_nonterminal_completeT
               (fst p)
-              (parse_name_or_abort G initial_names_data is_valid_name remove_name
-                                   remove_name_dec ntl_wf split_string_for_production
-                                   split_string_for_production_correct
-                                   p)
+              (parse_nonterminal_or_abort (G := G) p)
               (Pv p).
           Proof.
-            unfold parse_name_or_abort.
+            unfold parse_nonterminal_or_abort.
             let Acca := match goal with |- context[@Fix3 _ _ _ _ _ ?Rwf _ _ ?a] => constr:(Rwf a) end in
             induction (Acca) as [x ? IHr];
-              intros valid str pf name ?.
+              intros valid str pf nonterminal ?.
             rewrite Fix3_eq;
               [
               | solve [ intros;
-                        apply parse_name_step_ext;
+                        apply parse_nonterminal_step_ext;
                         trivial ] ].
             match goal with
               | [ H : appcontext[?f]
-                  |- _ -> parse_name_step _ _ _ _ _ _ _ (fun y _ b c d => ?f y b c d) _ _ _ = true ]
+                  |- _ -> parse_nonterminal_step (fun y _ b c d => ?f y b c d) _ _ _ = true ]
                 => revert H;
                   generalize f;
-                  let H' := fresh "parse_name_step'" in
+                  let H' := fresh "parse_nonterminal_step'" in
                   intros H' H
             end.
             destruct_head_hnf and.
-            intro; eapply parse_name_step_complete with (Pv := Pv); subst Pv;
+            intro; eapply parse_nonterminal_step_complete with (Pv := Pv); subst Pv;
             [ intros; eapply IHr | .. ];
             instantiate;
             trivial; simpl in *;
             try solve [ intros; reflexivity
                       | intros; split; reflexivity
                       | intros; split; try reflexivity;
-                        etransitivity; [ apply sub_names_listT_remove; assumption | assumption ] ].
+                        etransitivity; [ apply sub_names_listT_remove; assumption | assumption ] ];
+            [].
             { eapply expand_minimal_parse_of_name; [ .. | eassumption ];
               trivial;
               try reflexivity. }
           Defined.
 
-          Lemma parse_name_sound
-                (str : StringWithSplitState String split_stateT) (name : string)
-          : parse_name G initial_names_data is_valid_name remove_name
-                       remove_name_dec ntl_wf split_string_for_production
-                       split_string_for_production_correct
-                       str name
+          Lemma parse_nonterminal_sound
+                (str : StringWithSplitState String split_stateT) (nonterminal : string)
+          : parse_nonterminal (G := G) str nonterminal
             = true
-            -> parse_of_item _ G str (NonTerminal _ name).
+            -> parse_of_item _ G str (NonTerminal _ nonterminal).
           Proof.
-            unfold parse_name, parse_name_or_abort.
-            apply parse_name_or_abort_sound.
+            unfold parse_nonterminal, parse_nonterminal_or_abort.
+            apply parse_nonterminal_or_abort_sound.
           Defined.
 
-          Lemma parse_name_complete
-                (split_string_for_production_complete : forall str0 valid1 valid2 str pf prod, @split_list_completeT str0 valid1 valid2 str pf (split_string_for_production str prod) prod)
+          Lemma parse_nonterminal_complete
+                (split_string_for_production_complete : forall str0 valid str pf it its, @split_list_completeT str0 valid str pf (split_string_for_production it its str) (it::its))
                 (str : StringWithSplitState String split_stateT)
-                (name : string)
-          : minimal_parse_of_name String G initial_names_data is_valid_name remove_name str initial_names_data str name
-            -> parse_name G initial_names_data is_valid_name remove_name
-                          remove_name_dec ntl_wf split_string_for_production
-                          split_string_for_production_correct
-                          str name
+                (nonterminal : string)
+          : minimal_parse_of_name String G initial_nonterminals_data is_valid_nonterminal remove_nonterminal str initial_nonterminals_data str nonterminal
+            -> parse_nonterminal (G := G) str nonterminal
                = true.
           Proof.
-            unfold parse_name.
-            eapply (@parse_name_or_abort_complete
+            unfold parse_nonterminal.
+            eapply (@parse_nonterminal_or_abort_complete
                     split_string_for_production_complete
-                    (str, initial_names_data)).
+                    (str : String, initial_nonterminals_data)).
             split; reflexivity.
           Defined.
         End wf.
-      End names.
+      End nonterminals.
     End parts.
   End general.
 End sound.
@@ -655,7 +615,7 @@ Section brute_force_spliter.
   Qed.
 
   Lemma make_all_single_splits_complete
-  : forall G names_listT initial_names_data is_valid_name remove_name str0 valid0 valid1 str pf prod, @split_list_completeT _ string_stringlike G names_listT initial_names_data is_valid_name remove_name _ str0 valid0 valid1 str pf (@make_all_single_splits str) prod.
+  : forall G str0 valid str pf prod, @split_list_completeT _ string_stringlike G (brute_force_data G) str0 valid str pf (@make_all_single_splits str) prod.
   Proof.
     intros; hnf.
     destruct prod; trivial.
@@ -672,57 +632,55 @@ End brute_force_spliter.
 Section brute_force_make_parse_of.
   Variable G : grammar Ascii.ascii.
 
-  Definition brute_force_make_parse_of_sound
+  Definition brute_force_parse_sound
              (str : @String Ascii.ascii string_stringlike)
-             (name : string)
-  : brute_force_make_parse_of G str name = true -> parse_of_item _ G str (NonTerminal _ name).
+  : brute_force_parse G str = true -> parse_of_item _ G str (NonTerminal _ G).
   Proof.
-    unfold brute_force_make_parse_of.
-    apply parse_name_sound.
+    unfold brute_force_parse, brute_force_parse_nonterminal.
+    apply parse_nonterminal_sound.
   Defined.
 
-  Definition brute_force_make_parse_of_complete
+  Definition brute_force_parse_complete'
              (str : @String Ascii.ascii string_stringlike)
-             (name : string)
-  : minimal_parse_of_name _ G (Valid_nonterminal_symbols G) rdp_list_is_valid_name rdp_list_remove_name str (Valid_nonterminal_symbols G) str name
-    -> brute_force_make_parse_of G str name = true.
+  : minimal_parse_of_name _ G (Valid_nonterminals G) rdp_list_is_valid_nonterminal rdp_list_remove_nonterminal str (Valid_nonterminals G) str G
+    -> brute_force_parse G str = true.
   Proof.
-    unfold brute_force_make_parse_of; simpl; intro.
-    eapply parse_name_complete; try eassumption.
-    { apply rdp_list_remove_name_1. }
-    { apply rdp_list_remove_name_2. }
-    { apply make_all_single_splits_complete. }
+    unfold brute_force_parse, brute_force_parse_nonterminal.
+    simpl; intro.
+    eapply parse_nonterminal_complete; try eassumption.
+    { apply rdp_list_remove_nonterminal_1. }
+    { apply rdp_list_remove_nonterminal_2. }
+    { intros; apply make_all_single_splits_complete. }
   Defined.
 
-  Definition brute_force_make_parse_of_complete_p
+  Definition brute_force_parse_complete
              (str : @String Ascii.ascii string_stringlike)
-             (name : string)
-             (p : parse_of _ G str (Lookup G name))
-             (H_valid_name : rdp_list_is_valid_name (Valid_nonterminal_symbols G) name = true)
+             (p : parse_of _ G str G)
+             (H_valid_nonterminal : rdp_list_is_valid_nonterminal (Valid_nonterminals G) G = true)
              (H_valid_tree : Forall_parse_of
                                (fun _ p =>
-                                  rdp_list_is_valid_name (Valid_nonterminal_symbols G) p = true) p)
-  : brute_force_make_parse_of G str name = true.
+                                  rdp_list_is_valid_nonterminal (Valid_nonterminals G) p = true) p)
+  : brute_force_parse G str = true.
   Proof.
-    apply brute_force_make_parse_of_complete.
+    apply brute_force_parse_complete'.
     pose proof (@minimal_parse_of_name__of__parse_of_name
                   _ string_stringlike G
-                  rdp_list_names_listT
-                  (Valid_nonterminal_symbols G)
-                  rdp_list_is_valid_name rdp_list_remove_name
-                  rdp_list_remove_name_1
-                  rdp_list_remove_name_2
-                  (S (size_of_parse_item (ParseNonTerminal name p)))
+                  rdp_list_nonterminals_listT
+                  (Valid_nonterminals G)
+                  rdp_list_is_valid_nonterminal rdp_list_remove_nonterminal
+                  rdp_list_remove_nonterminal_1
+                  rdp_list_remove_nonterminal_2
+                  (S (size_of_parse_item (ParseNonTerminal G p)))
                   str str
-                  (Valid_nonterminal_symbols G)
-                  name
+                  (Valid_nonterminals G)
+                  G
                   p
                   (Lt.lt_n_Sn _)
                   (reflexivity _)
                   (reflexivity _)
-                  (H_valid_name, H_valid_tree))
+                  (H_valid_nonterminal, H_valid_tree))
       as p'.
-    destruct p' as [ [ p' ] | [ name' [ [ H0 H1 ] ] ] ].
+    destruct p' as [ [ p' ] | [ nonterminal' [ [ H0 H1 ] ] ] ].
     { exact p'. }
     { exfalso; congruence. }
   Qed.
