src/Parsers/DependentlyTyped.v
@@ -1,6 +1,6 @@
 (** * Definition of the interface and implementation of the dependently-typed CFG parser *)
 Require Import Coq.Lists.List Coq.Program.Program Coq.Program.Wf Coq.Arith.Wf_nat Coq.Arith.Compare_dec Coq.Classes.RelationClasses Coq.Strings.String.
-Require Import Parsers.ContextFreeGrammar.
+Require Import Parsers.ContextFreeGrammar Parsers.BaseTypes.
 Require Import Common Common.Wf.
 
 Set Implicit Arguments.
@@ -11,126 +11,32 @@ Local Coercion is_true : bool >-> Sortclass.
 
 (** TODO: Replace "name" with "nonterminal" *)
 
-Inductive any_grammar CharType :=
-| include_item (_ : item CharType)
-| include_production (_ : production CharType)
-| include_productions (_ : productions CharType)
-| include_nonterminal_name (_ : string).
-Global Coercion include_item : item >-> any_grammar.
-Global Coercion include_production : production >-> any_grammar.
-Global Coercion include_productions : productions >-> any_grammar.
-
 Section recursive_descent_parser.
   Context {CharType : Type}
           {String : string_like CharType}
           {G : grammar CharType}.
 
-  Class parser_computational_predataT :=
-    { nonterminal_names_listT : Type;
-      initial_nonterminal_names_data : nonterminal_names_listT;
-      is_valid_nonterminal_name : nonterminal_names_listT -> string -> bool;
-      remove_nonterminal_name : nonterminal_names_listT -> string -> nonterminal_names_listT;
-      nonterminal_names_listT_R : nonterminal_names_listT -> nonterminal_names_listT -> Prop;
-      remove_nonterminal_name_dec : forall ls nonterminal_name,
-                             is_valid_nonterminal_name ls nonterminal_name = true
-                             -> nonterminal_names_listT_R (remove_nonterminal_name ls nonterminal_name) ls;
-      ntl_wf : well_founded nonterminal_names_listT_R }.
-
-  Class parser_computational_types_dataT :=
-    { predata :> parser_computational_predataT;
-      split_stateT : String -> nonterminal_names_listT -> any_grammar CharType -> String -> Type }.
-
-  Class parser_computational_dataT' `{parser_computational_types_dataT} :=
-    { split_string_for_production
-      : forall (str0 : String) (valid : nonterminal_names_listT) (it : item CharType) (its : production CharType) (str : StringWithSplitState String (split_stateT str0 valid (it::its : production CharType))),
-          list (StringWithSplitState String (split_stateT str0 valid it)
-                * StringWithSplitState String (split_stateT str0 valid its));
-      split_string_for_production_correct
-      : forall str0 valid it its str,
-          let P f := List.Forall f (@split_string_for_production str0 valid it its str) in
-          P (fun s1s2 => (fst s1s2 ++ snd s1s2 =s str) = true) }.
-
-  Class parser_computational_dataT :=
-    { premethods :> parser_computational_types_dataT;
-      methods' :> parser_computational_dataT' }.
-
-  Class MonadT := Build_MonadT : Type -> Type.
-  Global Instance idM : MonadT | 10000 := fun x => x.
-  Global Strategy -1000 [idM].
-
-  Class parser_computational_prestrdataT `{parser_computational_dataT} `{M : MonadT} :=
-    { prelower_nonterminal_name_state
-      : forall {str0 valid nonterminal_name s},
-          split_stateT str0 valid (NonTerminal _ nonterminal_name) s -> M (split_stateT str0 valid (include_nonterminal_name _ nonterminal_name) s);
-
-      prelower_string_head
-      : forall {str0 valid}
-               {prod : production CharType}
-               {prods : productions CharType}
-               {s},
-          split_stateT str0 valid (prod::prods : productions CharType) s -> M (split_stateT str0 valid prod s);
-      prelower_string_tail
-      : forall {str0 valid}
-               {prod : production CharType}
-               {prods : productions CharType}
-               {s},
-          split_stateT str0 valid (prod::prods : productions CharType) s -> M (split_stateT str0 valid prods s);
-
-      prelift_lookup_nonterminal_name_state_lt
-      : forall {str0 valid nonterminal_name s} (pf : Length s < Length str0),
-          split_stateT str0 valid (include_nonterminal_name _ nonterminal_name) s -> M (split_stateT s initial_nonterminal_names_data (Lookup G nonterminal_name) s);
-
-      prelift_lookup_nonterminal_name_state_eq
-      : forall {str0 valid nonterminal_name s}
-               (pf : s = str0 :> String),
-          split_stateT str0 valid (include_nonterminal_name _ nonterminal_name) s -> M (split_stateT str0 (remove_nonterminal_name valid nonterminal_name) (Lookup G nonterminal_name) s) }.
-
-  Definition parser_computational_strdataT `{parser_computational_dataT} : Type
-    := parser_computational_prestrdataT.
-  Existing Class parser_computational_strdataT.
-
-  Definition lower_nonterminal_name_state `{methods : parser_computational_dataT, strdata : @parser_computational_strdataT methods}
-  : forall {str0 valid nonterminal_name s},
-      split_stateT _ _ _ _ -> split_stateT _ _ _ _
-    := @prelower_nonterminal_name_state methods (fun x => x) strdata.
-  Definition lower_string_head `{methods : parser_computational_dataT, strdata : @parser_computational_strdataT methods}
-  : forall {str0 valid prod prods s},
-      split_stateT _ _ _ _ -> split_stateT _ _ _ _
-    := @prelower_string_head methods (fun x => x) strdata.
-  Definition lower_string_tail `{methods : parser_computational_dataT, strdata : @parser_computational_strdataT methods}
-  : forall {str0 valid prod prods s},
-      split_stateT _ _ _ _ -> split_stateT _ _ _ _
-    := @prelower_string_tail methods (fun x => x) strdata.
-  Definition lift_lookup_nonterminal_name_state_lt `{methods : parser_computational_dataT, strdata : @parser_computational_strdataT methods}
-  : forall {str0 valid nonterminal_name s} pf,
-      split_stateT _ _ _ _ -> split_stateT _ _ _ _
-    := @prelift_lookup_nonterminal_name_state_lt methods (fun x => x) strdata.
-  Definition lift_lookup_nonterminal_name_state_eq `{methods : parser_computational_dataT, strdata : @parser_computational_strdataT methods}
-  : forall {str0 valid nonterminal_name s} pf,
-      split_stateT _ _ _ _ -> split_stateT _ _ _ _
-    := @prelift_lookup_nonterminal_name_state_eq methods (fun x => x) strdata.
-
   Section generic.
     Section parts.
-      Class parser_dependent_types_success_dataT' `{parser_computational_dataT} :=
-        { T_nonterminal_name_success
-          : forall (str0 : String) (valid : nonterminal_names_listT)
-                   (name : string)
-                   (str : StringWithSplitState String (split_stateT str0 valid (include_nonterminal_name _ name))),
+      Class parser_dependent_types_success_dataT' `{@parser_computational_dataT _ String} :=
+        { T_nonterminal_success
+          : forall (str0 : String) (valid : nonterminals_listT)
+                   (nt : string)
+                   (str : StringWithSplitState String (split_stateT str0 valid (include_nonterminal _ nt))),
               Type;
           T_item_success
-          : forall (str0 : String) (valid : nonterminal_names_listT)
+          : forall (str0 : String) (valid : nonterminals_listT)
                    (it : item CharType)
                    (str : StringWithSplitState String (split_stateT str0 valid it)),
               Type;
           T_production_success
-          : forall (str0 : String) (valid : nonterminal_names_listT)
+          : forall (str0 : String) (valid : nonterminals_listT)
                    (prod : production CharType)
                    (str : StringWithSplitState String (split_stateT str0 valid prod)),
               Type;
 
           T_productions_success
-          : forall (str0 : String) (valid : nonterminal_names_listT)
+          : forall (str0 : String) (valid : nonterminals_listT)
                    (prods : productions CharType)
                    (str : StringWithSplitState String (split_stateT str0 valid prods)),
               Type }.
@@ -140,24 +46,24 @@ Section recursive_descent_parser.
           stypes' :> parser_dependent_types_success_dataT' }.
 
       Class parser_dependent_types_failure_dataT' `{parser_dependent_types_success_dataT} :=
-        { T_nonterminal_name_failure
-          : forall (str0 : String) (valid : nonterminal_names_listT)
-                   (name : string)
-                   (str : StringWithSplitState String (split_stateT str0 valid (include_nonterminal_name _ name))),
+        { T_nonterminal_failure
+          : forall (str0 : String) (valid : nonterminals_listT)
+                   (nt : string)
+                   (str : StringWithSplitState String (split_stateT str0 valid (include_nonterminal _ nt))),
               Type;
           T_item_failure
-          : forall (str0 : String) (valid : nonterminal_names_listT)
+          : forall (str0 : String) (valid : nonterminals_listT)
                    (it : item CharType)
                    (str : StringWithSplitState String (split_stateT str0 valid it)),
               Type;
           T_production_failure
-          : forall (str0 : String) (valid : nonterminal_names_listT)
+          : forall (str0 : String) (valid : nonterminals_listT)
                    (prod : production CharType)
                    (str : StringWithSplitState String (split_stateT str0 valid prod)),
               Type;
 
           split_string_lift_T
-            (str0 : String) (valid : nonterminal_names_listT)
+            (str0 : String) (valid : nonterminals_listT)
             (it : item CharType) (its : production CharType)
             (str : StringWithSplitState String (split_stateT str0 valid (it::its : production CharType)))
             (split : list
@@ -177,7 +83,7 @@ Section recursive_descent_parser.
              -> T_production_failure str0 valid (it::its) str;
 
           T_productions_failure
-          : forall (str0 : String) (valid : nonterminal_names_listT)
+          : forall (str0 : String) (valid : nonterminals_listT)
                    (prods : productions CharType)
                    (str : StringWithSplitState String (split_stateT str0 valid prods)),
               Type }.
@@ -186,11 +92,11 @@ Section recursive_descent_parser.
         { stypes :> parser_dependent_types_success_dataT;
           ftypes' :> parser_dependent_types_failure_dataT' }.
 
-      Class parser_dependent_types_extra_success_dataT' `{types : parser_dependent_types_success_dataT, @parser_computational_strdataT (@methods types)} :=
+      Class parser_dependent_types_extra_success_dataT' `{types : parser_dependent_types_success_dataT, @parser_computational_strdataT _ _ _ (@methods types)} :=
         { lift_success
-          : forall {str0 valid} nonterminal_name {str},
-              @T_nonterminal_name_success _ _ str0 valid nonterminal_name (lift_StringWithSplitState str lower_nonterminal_name_state)
-              -> @T_item_success _ _ str0 valid (NonTerminal _ nonterminal_name) str;
+          : forall {str0 valid} nonterminal {str},
+              @T_nonterminal_success _ _ str0 valid nonterminal (lift_StringWithSplitState str lower_nonterminal_state)
+              -> @T_item_success _ _ str0 valid (NonTerminal _ nonterminal) str;
           parse_terminal_success
           : forall {str0 valid} ch {str},
               let ret := @T_item_success _ _ str0 valid (Terminal ch) str in
@@ -217,26 +123,26 @@ Section recursive_descent_parser.
               let arg := @T_productions_success _ _ str0 valid prods (lift_StringWithSplitState str lower_string_tail) in
               arg -> ret;
 
-          lift_parse_nonterminal_name_success_lt
-          : forall {str0 valid nonterminal_name str},
-              let ret := @T_nonterminal_name_success _ _ str0 valid nonterminal_name str in
+          lift_parse_nonterminal_success_lt
+          : forall {str0 valid nonterminal str},
+              let ret := @T_nonterminal_success _ _ str0 valid nonterminal str in
               forall (pf : Length str < Length str0),
-                let arg := @T_productions_success _ _ str initial_nonterminal_names_data (Lookup G nonterminal_name) (lift_StringWithSplitState str (lift_lookup_nonterminal_name_state_lt pf)) in
+                let arg := @T_productions_success _ _ str initial_nonterminals_data (Lookup G nonterminal) (lift_StringWithSplitState str (lift_lookup_nonterminal_state_lt pf)) in
                 arg -> ret;
-          lift_parse_nonterminal_name_success_eq
-          : forall {str0 valid nonterminal_name str},
-              let ret := @T_nonterminal_name_success _ _ str0 valid nonterminal_name str in
+          lift_parse_nonterminal_success_eq
+          : forall {str0 valid nonterminal str},
+              let ret := @T_nonterminal_success _ _ str0 valid nonterminal str in
               forall (pf : str = str0 :> String),
-                let arg := @T_productions_success _ _ str0 (remove_nonterminal_name valid nonterminal_name) (Lookup G nonterminal_name) (lift_StringWithSplitState str (lift_lookup_nonterminal_name_state_eq pf)) in
+                let arg := @T_productions_success _ _ str0 (remove_nonterminal valid nonterminal) (Lookup G nonterminal) (lift_StringWithSplitState str (lift_lookup_nonterminal_state_eq pf)) in
 
-                is_valid_nonterminal_name valid nonterminal_name = true -> arg -> ret
+                is_valid_nonterminal valid nonterminal = true -> arg -> ret
         }.
 
-      Class parser_dependent_types_extra_failure_dataT' `{types : parser_dependent_types_dataT, @parser_computational_strdataT (@methods (@stypes types))} :=
+      Class parser_dependent_types_extra_failure_dataT' `{types : parser_dependent_types_dataT, @parser_computational_strdataT _ _ _ (@methods (@stypes types))} :=
         { lift_failure
-          : forall {str0 valid} nonterminal_name {str},
-              @T_nonterminal_name_failure _ _ str0 valid nonterminal_name (lift_StringWithSplitState str lower_nonterminal_name_state)
-              -> @T_item_failure _ _ str0 valid (NonTerminal _ nonterminal_name) str;
+          : forall {str0 valid} nonterminal {str},
+              @T_nonterminal_failure _ _ str0 valid nonterminal (lift_StringWithSplitState str lower_nonterminal_state)
+              -> @T_item_failure _ _ str0 valid (NonTerminal _ nonterminal) str;
           parse_terminal_failure
           : forall {str0 valid} ch {str},
               let ret := @T_item_failure _ _ str0 valid (Terminal ch) str in
@@ -258,25 +164,25 @@ Section recursive_descent_parser.
           H_prod_split : forall str0 valid it its str, split_string_lift_T str0 valid it its str (split_string_for_production str0 valid it its str);
 
 
-          lift_parse_nonterminal_name_failure_lt
-          : forall {str0 valid nonterminal_name str},
-              let ret := @T_nonterminal_name_failure _ _ str0 valid nonterminal_name str in
+          lift_parse_nonterminal_failure_lt
+          : forall {str0 valid nonterminal str},
+              let ret := @T_nonterminal_failure _ _ str0 valid nonterminal str in
               forall (pf : Length str < Length str0),
-                let arg := @T_productions_failure _ _ str initial_nonterminal_names_data (Lookup G nonterminal_name) (lift_StringWithSplitState str (lift_lookup_nonterminal_name_state_lt pf)) in
+                let arg := @T_productions_failure _ _ str initial_nonterminals_data (Lookup G nonterminal) (lift_StringWithSplitState str (lift_lookup_nonterminal_state_lt pf)) in
                 arg -> ret;
-          lift_parse_nonterminal_name_failure_eq
-          : forall {str0 valid nonterminal_name str},
-              let ret := @T_nonterminal_name_failure _ _ str0 valid nonterminal_name str in
+          lift_parse_nonterminal_failure_eq
+          : forall {str0 valid nonterminal str},
+              let ret := @T_nonterminal_failure _ _ str0 valid nonterminal str in
               forall (pf : str = str0 :> String),
-                let arg := @T_productions_failure _ _ str0 (remove_nonterminal_name valid nonterminal_name) (Lookup G nonterminal_name) (lift_StringWithSplitState str (lift_lookup_nonterminal_name_state_eq pf)) in
+                let arg := @T_productions_failure _ _ str0 (remove_nonterminal valid nonterminal) (Lookup G nonterminal) (lift_StringWithSplitState str (lift_lookup_nonterminal_state_eq pf)) in
                 arg -> ret;
 
-          elim_parse_nonterminal_name_failure
-          : forall {str0 valid nonterminal_name str},
-              let ret := @T_nonterminal_name_failure _ _ str0 valid nonterminal_name str in
+          elim_parse_nonterminal_failure
+          : forall {str0 valid nonterminal str},
+              let ret := @T_nonterminal_failure _ _ str0 valid nonterminal str in
               str ≤s str0
               -> ~ Length str < Length str0
-              -> is_valid_nonterminal_name valid nonterminal_name = false
+              -> is_valid_nonterminal valid nonterminal = false
               -> ret
         }.
 
@@ -290,28 +196,28 @@ Section recursive_descent_parser.
 
       Section item.
         Context (str0 : String)
-                (valid : nonterminal_names_listT).
+                (valid : nonterminals_listT).
 
-        Let str_matches_nonterminal_nameT
+        Let str_matches_nonterminalT
             (str : String)
-          := forall nonterminal_name st,
+          := forall nonterminal st,
                let s := {| string_val := str ; state_val := st |} in
-               sum (T_nonterminal_name_success str0 valid nonterminal_name s)
-                   (T_nonterminal_name_failure str0 valid nonterminal_name s).
+               sum (T_nonterminal_success str0 valid nonterminal s)
+                   (T_nonterminal_failure str0 valid nonterminal s).
         Let T_item := fun it str => sum (T_item_success str0 valid it str) (T_item_failure str0 valid it str).
 
         Definition parse_item
                    (it : item CharType)
                    (str : StringWithSplitState String (split_stateT str0 valid it))
-                   (str_matches_nonterminal_name : str_matches_nonterminal_nameT str)
+                   (str_matches_nonterminal : str_matches_nonterminalT str)
         : T_item it str.
         Proof.
-          destruct it as [ ch | nonterminal_name ].
+          destruct it as [ ch | nonterminal ].
           { refine (if Sumbool.sumbool_of_bool ([[ ch ]] =s str)
                     then inl (parse_terminal_success ch _)
                     else inr (parse_terminal_failure ch _));
             assumption. }
-          { refine (if str_matches_nonterminal_name nonterminal_name _
+          { refine (if str_matches_nonterminal nonterminal _
                     then inl (lift_success _ _)
                     else inr (lift_failure _ _));
             eassumption. }
@@ -320,14 +226,14 @@ Section recursive_descent_parser.
 
       Section production_and_productions.
         Context (str0 : String)
-                (valid : nonterminal_names_listT).
+                (valid : nonterminals_listT).
 
-        Context (parse_nonterminal_name
+        Context (parse_nonterminal
                  : forall str,
                      str ≤s str0
-                     -> forall nonterminal_name st,
+                     -> forall nonterminal st,
                           let s := {| string_val := str ; state_val := st |} in
-                          sum (@T_nonterminal_name_success _ _ str0 valid nonterminal_name s) (@T_nonterminal_name_failure _ _ str0 valid nonterminal_name s)).
+                          sum (@T_nonterminal_success _ _ str0 valid nonterminal s) (@T_nonterminal_failure _ _ str0 valid nonterminal s)).
 
         Let T_production := fun prod str => sum (T_production_success str0 valid prod str) (T_production_failure str0 valid prod str).
 
@@ -367,7 +273,7 @@ Section recursive_descent_parser.
                                            valid
                                            it
                                            s1
-                                           (@parse_nonterminal_name s1 Hs1)),
+                                           (@parse_nonterminal s1 Hs1)),
                               (@parse_production s2 Hs2) with
                           | inl p_it, inl p_its => inl (@cons_success _ _ _ str0 valid _ _ _ s1 s2 pf _ _ _)
                           | inl p_it, inr p_its => parse_production_helper it its str pf splits _ parse_production _ _
@@ -441,65 +347,65 @@ Section recursive_descent_parser.
         End productions.
       End production_and_productions.
 
-      Section nonterminal_names.
+      Section nonterminals.
         Let T_productions := fun str0 valid prods str => sum (T_productions_success str0 valid prods str) (T_productions_failure str0 valid prods str).
 
-        Let T_nonterminal_name := fun str0 valid nonterminal_name str => sum (@T_nonterminal_name_success _ _ str0 valid nonterminal_name str) (@T_nonterminal_name_failure _ _ str0 valid nonterminal_name str).
+        Let T_nonterminal := fun str0 valid nonterminal str => sum (@T_nonterminal_success _ _ str0 valid nonterminal str) (@T_nonterminal_failure _ _ str0 valid nonterminal str).
 
         Section step.
           Context (str0 : String)
-                  (valid : nonterminal_names_listT).
+                  (valid : nonterminals_listT).
 
-          Context (parse_nonterminal_name
-                   : forall (p : String * nonterminal_names_listT),
-                       prod_relation (ltof _ Length) nonterminal_names_listT_R p (str0, valid)
-                       -> forall (nonterminal_name : string)
-                                 (str : StringWithSplitState String (split_stateT _ _ (include_nonterminal_name _ nonterminal_name)))
+          Context (parse_nonterminal
+                   : forall (p : String * nonterminals_listT),
+                       prod_relation (ltof _ Length) nonterminals_listT_R p (str0, valid)
+                       -> forall (nonterminal : string)
+                                 (str : StringWithSplitState String (split_stateT _ _ (include_nonterminal _ nonterminal)))
                                  (pf : str ≤s fst p),
-                            T_nonterminal_name (fst p) (snd p) nonterminal_name str).
+                            T_nonterminal (fst p) (snd p) nonterminal str).
 
-          Definition parse_nonterminal_name_step
-                     (nonterminal_name : string)
-                     (str : StringWithSplitState String (split_stateT _ _ (include_nonterminal_name _ nonterminal_name)))
+          Definition parse_nonterminal_step
+                     (nonterminal : string)
+                     (str : StringWithSplitState String (split_stateT _ _ (include_nonterminal _ nonterminal)))
                      (pf : str ≤s str0)
-          : T_nonterminal_name str0 valid nonterminal_name str.
+          : T_nonterminal str0 valid nonterminal str.
           Proof.
             refine (if lt_dec (Length str) (Length str0)
-                    then (** [str] got smaller, so we reset the valid nonterminal_names list *)
+                    then (** [str] got smaller, so we reset the valid nonterminals list *)
                       if (@parse_productions
                             _
                             _
-                            (fun str1 pf nonterminal_name st
-                             => @parse_nonterminal_name
-                                  (str : String, initial_nonterminal_names_data)
+                            (fun str1 pf nonterminal st
+                             => @parse_nonterminal
+                                  (str : String, initial_nonterminals_data)
                                   (or_introl _)
-                                  nonterminal_name
+                                  nonterminal
                                   {| string_val := str1 ; state_val := st |}
                                   pf)
-                            (Lookup G nonterminal_name)
-                            (lift_StringWithSplitState str (lift_lookup_nonterminal_name_state_lt _))
+                            (Lookup G nonterminal)
+                            (lift_StringWithSplitState str (lift_lookup_nonterminal_state_lt _))
                             (or_intror eq_refl))
-                      then inl (lift_parse_nonterminal_name_success_lt _ _)
-                      else inr (lift_parse_nonterminal_name_failure_lt _ _)
-                    else (** [str] didn't get smaller, so we cache the fact that we've hit this nonterminal_name already *)
-                      if Sumbool.sumbool_of_bool (is_valid_nonterminal_name valid nonterminal_name)
+                      then inl (lift_parse_nonterminal_success_lt _ _)
+                      else inr (lift_parse_nonterminal_failure_lt _ _)
+                    else (** [str] didn't get smaller, so we cache the fact that we've hit this nonterminal already *)
+                      if Sumbool.sumbool_of_bool (is_valid_nonterminal valid nonterminal)
                       then (** It was valid, so we can remove it *)
                         if (@parse_productions
                               _ _
-                              (fun str1 (pf : str1 ≤s str0) nonterminal_name' st
-                               => @parse_nonterminal_name
-                                    (str0, remove_nonterminal_name valid nonterminal_name)
-                                    (or_intror (conj eq_refl (@remove_nonterminal_name_dec _ _ _ _)))
-                                    nonterminal_name'
+                              (fun str1 (pf : str1 ≤s str0) nonterminal' st
+                               => @parse_nonterminal
+                                    (str0, remove_nonterminal valid nonterminal)
+                                    (or_intror (conj eq_refl (@remove_nonterminal_dec _ _ _ _)))
+                                    nonterminal'
                                     {| string_val := str1 ; state_val := st |}
                                     pf)
-                              (Lookup G nonterminal_name)
-                              (lift_StringWithSplitState str (lift_lookup_nonterminal_name_state_eq (or_not_l pf _)))
+                              (Lookup G nonterminal)
+                              (lift_StringWithSplitState str (lift_lookup_nonterminal_state_eq (or_not_l pf _)))
                               (or_intror _))
-                        then inl (lift_parse_nonterminal_name_success_eq _ _ _)
-                        else inr (lift_parse_nonterminal_name_failure_eq _ _)
-                      else (** oops, we already saw this nonterminal_name in the past.  ABORT! *)
-                        inr (elim_parse_nonterminal_name_failure _ _ _));
+                        then inl (lift_parse_nonterminal_success_eq _ _ _)
+                        else inr (lift_parse_nonterminal_failure_eq _ _)
+                      else (** oops, we already saw this nonterminal in the past.  ABORT! *)
+                        inr (elim_parse_nonterminal_failure _ _ _));
             try solve [ pre_eassumption; instantiate_evars; eassumption
                       | destruct_head_hnf or; try assumption; exfalso; eauto with nocore ].
           Defined.
@@ -507,37 +413,37 @@ Section recursive_descent_parser.
 
         Section wf.
           (** TODO: add comment explaining signature *)
-          Definition parse_nonterminal_name_or_abort
-          : forall (p : String * nonterminal_names_listT)
-                   (nonterminal_name : string)
-                   (str : StringWithSplitState String (split_stateT _ _ (include_nonterminal_name _ nonterminal_name)))
+          Definition parse_nonterminal_or_abort
+          : forall (p : String * nonterminals_listT)
+                   (nonterminal : string)
+                   (str : StringWithSplitState String (split_stateT _ _ (include_nonterminal _ nonterminal)))
                    (pf : str ≤s fst p),
-              T_nonterminal_name (fst p) (snd p) nonterminal_name str
+              T_nonterminal (fst p) (snd p) nonterminal str
             := @Fix3
-                 (prod String nonterminal_names_listT) _ _ _
+                 (prod String nonterminals_listT) _ _ _
                  _ (@well_founded_prod_relation
                       String
-                      nonterminal_names_listT
+                      nonterminals_listT
                       _
                       _
                       (well_founded_ltof _ Length)
                       ntl_wf)
                  _
-                 (fun sl => @parse_nonterminal_name_step (fst sl) (snd sl)).
+                 (fun sl => @parse_nonterminal_step (fst sl) (snd sl)).
 
-          Definition parse_nonterminal_name
-                     (nonterminal_name : string)
+          Definition parse_nonterminal
+                     (nonterminal : string)
                      (s : String)
-                     (st : split_stateT s _ (include_nonterminal_name _ nonterminal_name) s)
+                     (st : split_stateT s _ (include_nonterminal _ nonterminal) s)
                      (str := {| string_val := s ; state_val := st |})
-          : T_nonterminal_name str initial_nonterminal_names_data nonterminal_name str
-            := @parse_nonterminal_name_or_abort
-                 (str : String, initial_nonterminal_names_data)
-                 nonterminal_name
+          : T_nonterminal str initial_nonterminals_data nonterminal str
+            := @parse_nonterminal_or_abort
+                 (str : String, initial_nonterminals_data)
+                 nonterminal
                  str
                  (or_intror eq_refl).
         End wf.
-      End nonterminal_names.
+      End nonterminals.
     End parts.
   End generic.
 End recursive_descent_parser.
