src/Parsers/DependentlyTypedMinimalOfParse.v
@@ -1,7 +1,7 @@
 (** * Specialization of the dependently typed parser to minimal parse trees, taking in parse trees *)
 Require Import Coq.Lists.List Coq.Program.Program Coq.Program.Wf Coq.Arith.Wf_nat Coq.Arith.Compare_dec Coq.Classes.RelationClasses Coq.Strings.String.
 Require Import Parsers.ContextFreeGrammar Parsers.DependentlyTyped Parsers.MinimalParse.
-Require Import Parsers.WellFoundedParse Parsers.ContextFreeGrammarProperties.
+Require Import Parsers.WellFoundedParse Parsers.ContextFreeGrammarProperties Parsers.BaseTypes.
 Require Import Common Common.Wf Common.Le.
 
 Set Implicit Arguments.
@@ -18,29 +18,29 @@ Section recursive_descent_parser.
   Local Instance types_methods : @parser_computational_types_dataT _ String
     := { predata := premethods;
          split_stateT str0 valid g str := unit }.
-  Context (remove_nonterminal_name_1
+  Context (remove_nonterminal_1
            : forall ls ps ps',
-               is_valid_nonterminal_name (remove_nonterminal_name ls ps) ps' = true
-               -> is_valid_nonterminal_name ls ps' = true)
-          (remove_nonterminal_name_2
+               is_valid_nonterminal (remove_nonterminal ls ps) ps' = true
+               -> is_valid_nonterminal ls ps' = true)
+          (remove_nonterminal_2
            : forall ls ps ps',
-               is_valid_nonterminal_name (remove_nonterminal_name ls ps) ps' = false
-               <-> is_valid_nonterminal_name ls ps' = false \/ ps = ps').
+               is_valid_nonterminal (remove_nonterminal ls ps) ps' = false
+               <-> is_valid_nonterminal ls ps' = false \/ ps = ps').
   Variable orig_methods : @parser_computational_dataT' CharType String types_methods.
 
   Definition P (str0 : String) valid : String -> string -> Prop
     := fun str p =>
-         sub_names_listT is_valid_nonterminal_name valid initial_nonterminal_names_data
-         /\ is_valid_nonterminal_name
+         sub_names_listT is_valid_nonterminal valid initial_nonterminals_data
+         /\ is_valid_nonterminal
               (if lt_dec (Length str) (Length str0)
-               then initial_nonterminal_names_data
+               then initial_nonterminals_data
                else valid)
               p = true.
 
   Lemma P_remove_impl {str0 valid str name name'}
         (H0 : name <> name')
         (H : P str0 valid str name')
-  : P str0 (remove_nonterminal_name valid name) str name'.
+  : P str0 (remove_nonterminal valid name) str name'.
   Proof.
     destruct_head_hnf and.
     repeat split; try assumption.
@@ -50,7 +50,7 @@ Section recursive_descent_parser.
         | [ |- ?b = true ] => case_eq b; try reflexivity
       end.
       intro H'; exfalso.
-      apply remove_nonterminal_name_2 in H'.
+      apply remove_nonterminal_2 in H'.
       destruct H'; congruence. }
   Qed.
 
@@ -60,17 +60,17 @@ Section recursive_descent_parser.
     := { p' : parse_of_production String G s p & Forall_parse_of_production (P str0 valid) p' }.
   Definition p_parse str0 valid s prods
     := { p' : parse_of String G s prods & Forall_parse_of (P str0 valid) p' }.
-  Definition p_parse_nonterminal_name str0 valid s nonterminal_name
-    := { p' : parse_of_item String G  s (NonTerminal _ nonterminal_name) & Forall_parse_of_item (P str0 valid) p' }.
+  Definition p_parse_nonterminal str0 valid s nonterminal
+    := { p' : parse_of_item String G  s (NonTerminal _ nonterminal) & Forall_parse_of_item (P str0 valid) p' }.
 
   Definition mp_parse_item str0 valid str it
-    := minimal_parse_of_item String G initial_nonterminal_names_data is_valid_nonterminal_name remove_nonterminal_name str0 valid str it.
+    := minimal_parse_of_item String G initial_nonterminals_data is_valid_nonterminal remove_nonterminal str0 valid str it.
   Definition mp_parse_production str0 valid str prod
-    := minimal_parse_of_production String G initial_nonterminal_names_data is_valid_nonterminal_name remove_nonterminal_name str0 valid str prod.
+    := minimal_parse_of_production String G initial_nonterminals_data is_valid_nonterminal remove_nonterminal str0 valid str prod.
   Definition mp_parse str0 valid str prods
-    := minimal_parse_of String G initial_nonterminal_names_data is_valid_nonterminal_name remove_nonterminal_name str0 valid str prods.
-  Definition mp_parse_nonterminal_name str0 valid str nonterminal_name
-    := minimal_parse_of_name String G initial_nonterminal_names_data is_valid_nonterminal_name remove_nonterminal_name str0 valid str nonterminal_name.
+    := minimal_parse_of String G initial_nonterminals_data is_valid_nonterminal remove_nonterminal str0 valid str prods.
+  Definition mp_parse_nonterminal str0 valid str nonterminal
+    := minimal_parse_of_name String G initial_nonterminals_data is_valid_nonterminal remove_nonterminal str0 valid str nonterminal.
 
   Definition split_parse_of_production {str0 valid str it its}
              (p : p_parse_production str0 valid str (it::its))
@@ -121,7 +121,7 @@ Section recursive_descent_parser.
                       | include_item it => p_parse_item str0 valid s it
                       | include_production p => p_parse_production str0 valid s p
                       | include_productions prods => p_parse str0 valid s prods
-                      | include_nonterminal_name nonterminal_name => p_parse_nonterminal_name str0 valid s nonterminal_name
+                      | include_nonterminal nonterminal => p_parse_nonterminal str0 valid s nonterminal
                     end) }.
 
   Local Instance methods' : @parser_computational_dataT' _ String types_methods'
@@ -156,15 +156,15 @@ Section recursive_descent_parser.
       ).
   Defined.
 
-  Definition parse_of__of__parse_of_item_lt' {str0 valid str nonterminal_name}
+  Definition parse_of__of__parse_of_item_lt' {str0 valid str nonterminal}
              (pf : Length str < Length str0)
-             (p : p_parse_nonterminal_name str0 valid str nonterminal_name)
-  : P str0 valid str nonterminal_name * p_parse str initial_nonterminal_names_data str (Lookup G nonterminal_name).
+             (p : p_parse_nonterminal str0 valid str nonterminal)
+  : P str0 valid str nonterminal * p_parse str initial_nonterminals_data str (Lookup G nonterminal).
   Proof.
     refine (match projT1 p as p' in parse_of_item _ _ str' it'
                   return match it' with
                            | Terminal _ => True
-                           | NonTerminal nonterminal_name' => Length str' < Length str0 -> Forall_parse_of_item (P str0 valid) p' -> P str0 valid str' nonterminal_name' * p_parse str' initial_nonterminal_names_data str' (Lookup G nonterminal_name')
+                           | NonTerminal nonterminal' => Length str' < Length str0 -> Forall_parse_of_item (P str0 valid) p' -> P str0 valid str' nonterminal' * p_parse str' initial_nonterminals_data str' (Lookup G nonterminal')
                          end
             with
               | ParseTerminal _ => I
@@ -173,46 +173,46 @@ Section recursive_descent_parser.
     clear -pf'; unfold P in *; simpl;
     abstract (intros ??; do 2 edestruct lt_dec; intuition).
   Defined.
-  Definition parse_of__of__parse_of_item_lt {str0 valid str nonterminal_name} pf p
-    := snd (@parse_of__of__parse_of_item_lt' str0 valid str nonterminal_name pf p).
+  Definition parse_of__of__parse_of_item_lt {str0 valid str nonterminal} pf p
+    := snd (@parse_of__of__parse_of_item_lt' str0 valid str nonterminal pf p).
 
-  Definition deloop_right str0 valid str nonterminal_name
-    := p_parse str0 (remove_nonterminal_name valid nonterminal_name) str (Lookup G nonterminal_name).
+  Definition deloop_right str0 valid str nonterminal
+    := p_parse str0 (remove_nonterminal valid nonterminal) str (Lookup G nonterminal).
 
   Definition deloop_onceT
-    := forall str0 valid str nonterminal_name prods
+    := forall str0 valid str nonterminal prods
               (p : parse_of String G str prods)
               (pf : str = str0 :> String)
               (H : Forall_parse_of (P str0 valid) p),
-         p_parse str0 (remove_nonterminal_name valid nonterminal_name) str prods
-         + deloop_right str0 valid str nonterminal_name.
+         p_parse str0 (remove_nonterminal valid nonterminal) str prods
+         + deloop_right str0 valid str nonterminal.
 
   Definition deloop_once_productionT
-    := forall str0 valid str nonterminal_name prod
+    := forall str0 valid str nonterminal prod
               (p : parse_of_production String G str prod)
               (pf : str = str0 :> String)
               (H : Forall_parse_of_production (P str0 valid) p),
-         p_parse_production str0 (remove_nonterminal_name valid nonterminal_name) str prod
-         + deloop_right str0 valid str nonterminal_name.
+         p_parse_production str0 (remove_nonterminal valid nonterminal) str prod
+         + deloop_right str0 valid str nonterminal.
 
   Definition deloop_once_item'
              (deloop_once : deloop_onceT)
-             {str0 valid str nonterminal_name}
+             {str0 valid str nonterminal}
              {it}
              (p : parse_of_item String G str it)
              (pf : str = str0 :> String)
              (H : Forall_parse_of_item (P str0 valid) p)
-  : p_parse_item str0 (remove_nonterminal_name valid nonterminal_name) str it
-    + deloop_right str0 valid str nonterminal_name.
+  : p_parse_item str0 (remove_nonterminal valid nonterminal) str it
+    + deloop_right str0 valid str nonterminal.
   Proof.
-    destruct p as [ | nonterminal_name' str'' p' ].
+    destruct p as [ | nonterminal' str'' p' ].
     { exact (inl (existT _ (ParseTerminal _ _ _) tt)). }
-    { refine (if string_dec nonterminal_name nonterminal_name'
-              then inr match @deloop_once _ _ _ nonterminal_name' _ p' pf (snd H) with
+    { refine (if string_dec nonterminal nonterminal'
+              then inr match @deloop_once _ _ _ nonterminal' _ p' pf (snd H) with
                          | inl p''' => _
                          | inr ret => _
                        end
-              else match @deloop_once _ _ _ nonterminal_name _ p' pf (snd H) with
+              else match @deloop_once _ _ _ nonterminal _ p' pf (snd H) with
                      | inl p''' => inl (existT _ (ParseNonTerminal _ (projT1 p''')) (P_remove_impl _ (fst H), projT2 p'''))
                      | inr ret => inr ret
                    end);
@@ -226,13 +226,13 @@ Section recursive_descent_parser.
              (deloop_once_production : deloop_once_productionT)
   : deloop_onceT.
   Proof.
-    intros str0 valid str nonterminal_name pats p pf H.
+    intros str0 valid str nonterminal pats p pf H.
     destruct p as [ str' pat' pats' p' | str' pat' pats' p' ].
-    { refine match deloop_once_production str0 valid str' nonterminal_name _ p' pf H with
+    { refine match deloop_once_production str0 valid str' nonterminal _ p' pf H with
                | inl ret => inl (existT _ (ParseHead pats' (projT1 ret)) (projT2 ret))
                | inr ret => inr ret
              end. }
-    { refine match deloop_once str0 valid str' nonterminal_name _ p' pf H with
+    { refine match deloop_once str0 valid str' nonterminal _ p' pf H with
                | inl ret => inl (existT _ (ParseTail _ (projT1 ret)) (projT2 ret))
                | inr ret => inr ret
              end. }
@@ -251,7 +251,7 @@ Section recursive_descent_parser.
              | [ H : _ < 0 |- _ ] => destruct (Lt.lt_n_0 _ H)
              | _ => progress destruct_head and
              | [ |- _ /\ _ ] => split
-             | [ H : sub_names_listT _ _ _ |- is_valid_nonterminal_name _ _ = true ]
+             | [ H : sub_names_listT _ _ _ |- is_valid_nonterminal _ _ = true ]
                => (apply H; eapply sub_names_listT_remove; eassumption)
              | [ H : ~0 < ?n |- _ ]
                => (let H' := fresh in
@@ -273,18 +273,18 @@ Section recursive_descent_parser.
              (deloop_once_production : deloop_once_productionT)
   : deloop_once_productionT.
   Proof.
-    intros str0 valid str nonterminal_name pat p pf H.
+    intros str0 valid str nonterminal pat p pf H.
     destruct p as [ | str' pat' strs' pats' p' p'' ].
     { refine (inl (existT _ (ParseProductionNil _ _) tt)). }
     { (** We must discriminate based on whether or not [str] has already gotten shorter *)
       destruct (stringlike_dec str' (Empty _)) as [e|e], (stringlike_dec strs' (Empty _)) as [e'|e'];
       try (assert (pf0 : str' = str0)
             by (clear -pf e'; abstract (subst strs'; rewrite ?RightId, ?LeftId in pf; exact pf));
-           pose proof (@deloop_once_item' (deloop_once) str0 valid _ nonterminal_name pat' p' pf0 (fst H)) as deloop_once_item;
+           pose proof (@deloop_once_item' (deloop_once) str0 valid _ nonterminal pat' p' pf0 (fst H)) as deloop_once_item;
            clear deloop_once);
       try (assert (pf1 : strs' = str0)
             by (clear -pf e; abstract (subst str'; rewrite ?RightId, ?LeftId in pf; exact pf));
-           specialize (deloop_once_production str0 valid _ nonterminal_name pats' p'' pf1 (snd H)));
+           specialize (deloop_once_production str0 valid _ nonterminal pats' p'' pf1 (snd H)));
       try (destruct deloop_once_item as [ret|ret];
            [ | right; repeat first [ subst str' | subst strs' ]; rewrite ?LeftId, ?RightId; assumption ]);
       try (destruct deloop_once_production as [ret'|ret'];
@@ -298,14 +298,14 @@ Section recursive_descent_parser.
         exists (ParseProductionCons p' (projT1 ret')).
         refine (expand_forall_parse_of_item _ (fst H), projT2 ret').
         unfold P in *; simpl.
-        clear -e e' pf1 remove_nonterminal_name_1 remove_nonterminal_name_2.
+        clear -e e' pf1 remove_nonterminal_1 remove_nonterminal_2.
         abstract (intros; edestruct lt_dec; deloop_t). }
       { (** nonempty, empty *)
         left.
         exists (ParseProductionCons (projT1 ret) p'').
         refine (projT2 ret, expand_forall_parse_of_production _ _ (snd H)).
         unfold P in *; simpl.
-        clear -e e' pf0 remove_nonterminal_name_1 remove_nonterminal_name_2.
+        clear -e e' pf0 remove_nonterminal_1 remove_nonterminal_2.
         abstract (intros; edestruct lt_dec; deloop_t). }
       { (** nonempty, nonempty *)
         left.
@@ -313,42 +313,42 @@ Section recursive_descent_parser.
         refine (expand_forall_parse_of_item _ (fst H),
                 expand_forall_parse_of_production _ _ (snd H));
           unfold P in *; simpl;
-          clear -e e' pf remove_nonterminal_name_1 remove_nonterminal_name_2;
+          clear -e e' pf remove_nonterminal_1 remove_nonterminal_2;
           abstract (intros; edestruct lt_dec; deloop_t). } }
   Defined.
 
-  Fixpoint deloop_once {str0 valid str nonterminal_name pats} (p : parse_of String G str pats)
-    := @deloop_once' (@deloop_once) (@deloop_once_production) str0 valid str nonterminal_name pats p
-  with deloop_once_production {str0 valid str nonterminal_name pat} (p : parse_of_production String G str pat)
-       := @deloop_once_production' (@deloop_once) (@deloop_once_production) str0 valid str nonterminal_name pat p.
-  Definition deloop_once_item {str0 valid str nonterminal_name it} (p : parse_of_item String G str it)
-    := @deloop_once_item' (@deloop_once) str0 valid str nonterminal_name it p.
+  Fixpoint deloop_once {str0 valid str nonterminal pats} (p : parse_of String G str pats)
+    := @deloop_once' (@deloop_once) (@deloop_once_production) str0 valid str nonterminal pats p
+  with deloop_once_production {str0 valid str nonterminal pat} (p : parse_of_production String G str pat)
+       := @deloop_once_production' (@deloop_once) (@deloop_once_production) str0 valid str nonterminal pat p.
+  Definition deloop_once_item {str0 valid str nonterminal it} (p : parse_of_item String G str it)
+    := @deloop_once_item' (@deloop_once) str0 valid str nonterminal it p.
 
-  Definition parse_of__of__parse_of_item_eq' {str0 valid str nonterminal_name}
+  Definition parse_of__of__parse_of_item_eq' {str0 valid str nonterminal}
              (pf : str = str0 :> String)
-             (p : p_parse_nonterminal_name str0 valid str nonterminal_name)
-  : P str0 valid str nonterminal_name * p_parse str0 (remove_nonterminal_name valid nonterminal_name) str (Lookup G nonterminal_name).
+             (p : p_parse_nonterminal str0 valid str nonterminal)
+  : P str0 valid str nonterminal * p_parse str0 (remove_nonterminal valid nonterminal) str (Lookup G nonterminal).
   Proof.
     refine (match projT1 p as p' in parse_of_item _ _ str' it'
                   return match it' with
                            | Terminal _ => True
-                           | NonTerminal nonterminal_name' => str' = str0 -> Forall_parse_of_item (P str0 valid) p' -> P str0 valid str' nonterminal_name' * p_parse str0 (remove_nonterminal_name valid nonterminal_name') str' (Lookup G nonterminal_name')
+                           | NonTerminal nonterminal' => str' = str0 -> Forall_parse_of_item (P str0 valid) p' -> P str0 valid str' nonterminal' * p_parse str0 (remove_nonterminal valid nonterminal') str' (Lookup G nonterminal')
                          end
             with
               | ParseTerminal _ => I
-              | ParseNonTerminal nonterminal_name' _ p'
-                => fun pf' H' => (fst H', if @deloop_once str0 valid _ nonterminal_name' _ p' pf' (snd H') then _ else _)
+              | ParseNonTerminal nonterminal' _ p'
+                => fun pf' H' => (fst H', if @deloop_once str0 valid _ nonterminal' _ p' pf' (snd H') then _ else _)
             end pf (projT2 p));
     assumption.
   Defined.
-  Definition parse_of__of__parse_of_item_eq {str0 valid str nonterminal_name} pf p
-    := snd (@parse_of__of__parse_of_item_eq' str0 valid str nonterminal_name pf p).
+  Definition parse_of__of__parse_of_item_eq {str0 valid str nonterminal} pf p
+    := snd (@parse_of__of__parse_of_item_eq' str0 valid str nonterminal pf p).
 
   Local Instance methods : @parser_computational_dataT _ String
     := { methods' := methods' }.
 
   Local Instance prestrdata : @parser_computational_prestrdataT _ String G methods idM
-    := { prelower_nonterminal_name_state str0 valid nonterminal_name str st := st;
+    := { prelower_nonterminal_state str0 valid nonterminal str st := st;
          prelower_string_head str0 valid prod prods str st
          := match st with
               | None => None
@@ -365,8 +365,8 @@ Section recursive_descent_parser.
                             | ParseHead _ _ _ _ => fun _ => None
                           end (projT2 p)
             end;
-         prelift_lookup_nonterminal_name_state_lt str0 valid nonterminal_name str pf := option_map (parse_of__of__parse_of_item_lt pf);
-         prelift_lookup_nonterminal_name_state_eq str0 valid nonterminal_name str pf := option_map (parse_of__of__parse_of_item_eq pf) }.
+         prelift_lookup_nonterminal_state_lt str0 valid nonterminal str pf := option_map (parse_of__of__parse_of_item_lt pf);
+         prelift_lookup_nonterminal_state_eq str0 valid nonterminal str pf := option_map (parse_of__of__parse_of_item_eq pf) }.
 
   Local Instance strdata : @parser_computational_strdataT _ String G methods
     := prestrdata.
@@ -396,27 +396,27 @@ Section recursive_descent_parser.
       Section common.
         Section types.
           Context (str0 : String)
-                  (valid : nonterminal_names_listT).
+                  (valid : nonterminals_listT).
 
           Let prefix str T := str ≤s str0
-                              -> sub_names_listT is_valid_nonterminal_name valid initial_nonterminal_names_data
+                              -> sub_names_listT is_valid_nonterminal valid initial_nonterminals_data
                               -> T.
 
           Let alt := False.
 
-          Section T_nonterminal_name.
-            Context (name : string) (str : StringWithSplitState String (split_stateT str0 valid (include_nonterminal_name _ name))).
-            Let ret := mp_parse_nonterminal_name str0 valid str name.
+          Section T_nonterminal.
+            Context (name : string) (str : StringWithSplitState String (split_stateT str0 valid (include_nonterminal _ name))).
+            Let ret := mp_parse_nonterminal str0 valid str name.
 
-            Definition T_nonterminal_name_success  : Type
+            Definition T_nonterminal_success  : Type
               := ret.
 
-            Definition T_nonterminal_name_failure : Type
+            Definition T_nonterminal_failure : Type
               := match state_val str with
                    | None => ret -> False
                    | Some p => alt
                  end.
-          End T_nonterminal_name.
+          End T_nonterminal.
 
           Section T_item.
             Context (it : item CharType) (str : StringWithSplitState String (split_stateT str0 valid it)).
@@ -464,7 +464,7 @@ Section recursive_descent_parser.
 
         Global Instance minimal_parser_dependent_types_success_data'
         : @parser_dependent_types_success_dataT' _ String _
-          := { T_nonterminal_name_success := T_nonterminal_name_success;
+          := { T_nonterminal_success := T_nonterminal_success;
                T_item_success := T_item_success;
                T_production_success := T_production_success;
                T_productions_success := T_productions_success }.
@@ -475,7 +475,7 @@ Section recursive_descent_parser.
 
         Global Instance minimal_parser_dependent_types_failure_data'
         : @parser_dependent_types_failure_dataT' _ String _
-          := { T_nonterminal_name_failure := T_nonterminal_name_failure;
+          := { T_nonterminal_failure := T_nonterminal_failure;
                T_item_failure := T_item_failure;
                T_production_failure := T_production_failure;
                T_productions_failure := T_productions_failure }.
@@ -486,10 +486,10 @@ Section recursive_descent_parser.
                ftypes' := minimal_parser_dependent_types_failure_data' }.
 
         Hint Constructors minimal_parse_of minimal_parse_of_name minimal_parse_of_production minimal_parse_of_item unit prod unit : minimal_instance_db.
-        Hint Unfold T_item_success T_item_failure T_production_success T_production_failure T_productions_success T_productions_failure T_nonterminal_name_success T_nonterminal_name_failure
-             DependentlyTyped.T_item_success DependentlyTyped.T_item_failure DependentlyTyped.T_production_success DependentlyTyped.T_production_failure DependentlyTyped.T_productions_success DependentlyTyped.T_productions_failure DependentlyTyped.T_nonterminal_name_success DependentlyTyped.T_nonterminal_name_failure
-             p_parse_production p_parse p_parse_item p_parse_nonterminal_name
-             mp_parse_production mp_parse mp_parse_item mp_parse_nonterminal_name : minimal_instance_db.
+        Hint Unfold T_item_success T_item_failure T_production_success T_production_failure T_productions_success T_productions_failure T_nonterminal_success T_nonterminal_failure
+             DependentlyTyped.T_item_success DependentlyTyped.T_item_failure DependentlyTyped.T_production_success DependentlyTyped.T_production_failure DependentlyTyped.T_productions_success DependentlyTyped.T_productions_failure DependentlyTyped.T_nonterminal_success DependentlyTyped.T_nonterminal_failure
+             p_parse_production p_parse p_parse_item p_parse_nonterminal
+             mp_parse_production mp_parse mp_parse_item mp_parse_nonterminal : minimal_instance_db.
 
         Local Ltac t''0 :=
           first [ progress cbv zeta
@@ -681,19 +681,19 @@ Please report." *)
       End common.
     End parts.
 
-    Definition minimal_parse_nonterminal_name__of__parse
+    Definition minimal_parse_nonterminal__of__parse
                (H_prod_split' : forall str0 valid it its str, @H_prod_splitT' str0 valid it its str None)
-               (nonterminal_name : string)
+               (nonterminal : string)
                (s : String)
-               (p : parse_of_item String G s (NonTerminal _ nonterminal_name))
+               (p : parse_of_item String G s (NonTerminal _ nonterminal))
                (H : Forall_parse_of_item
-                      (fun _ n => is_valid_nonterminal_name initial_nonterminal_names_data n = true)
+                      (fun _ n => is_valid_nonterminal initial_nonterminals_data n = true)
                       p)
-    : minimal_parse_of_name String G initial_nonterminal_names_data is_valid_nonterminal_name remove_nonterminal_name s initial_nonterminal_names_data s nonterminal_name.
+    : minimal_parse_of_name String G initial_nonterminals_data is_valid_nonterminal remove_nonterminal s initial_nonterminals_data s nonterminal.
     Proof.
-      pose proof (fun H' => @parse_nonterminal_name _ String G (minimal_parser_dependent_types_extra_data H_prod_split') nonterminal_name s (Some (existT _ p (expand_forall_parse_of_item H' H)))) as H0.
+      pose proof (fun H' => @parse_nonterminal _ String G (minimal_parser_dependent_types_extra_data H_prod_split') nonterminal s (Some (existT _ p (expand_forall_parse_of_item H' H)))) as H0.
       simpl in *.
-      unfold T_nonterminal_name_success, T_nonterminal_name_failure in *.
+      unfold T_nonterminal_success, T_nonterminal_failure in *.
       simpl in *.
       edestruct H0; unfold P;
         repeat match goal with
