src/Parsers/BaseTypes.v
@@ -1,0 +1,111 @@
+(** * Definition of the common part of the interface of the CFG parser *)
+Require Import Coq.Lists.List Coq.Init.Wf Coq.Strings.String.
+Require Import Parsers.ContextFreeGrammar.
+
+Set Implicit Arguments.
+
+Local Open Scope string_like_scope.
+
+Local Coercion is_true : bool >-> Sortclass.
+
+Inductive any_grammar CharType :=
+| include_item (_ : item CharType)
+| include_production (_ : production CharType)
+| include_productions (_ : productions CharType)
+| include_nonterminal (_ : string).
+Global Coercion include_item : item >-> any_grammar.
+Global Coercion include_production : production >-> any_grammar.
+Global Coercion include_productions : productions >-> any_grammar.
+
+Section recursive_descent_parser.
+  Context {CharType : Type}
+          {String : string_like CharType}
+          {G : grammar CharType}.
+
+  Class parser_computational_predataT :=
+    { nonterminals_listT : Type;
+      initial_nonterminals_data : nonterminals_listT;
+      is_valid_nonterminal : nonterminals_listT -> string -> bool;
+      remove_nonterminal : nonterminals_listT -> string -> nonterminals_listT;
+      nonterminals_listT_R : nonterminals_listT -> nonterminals_listT -> Prop;
+      remove_nonterminal_dec : forall ls nonterminal,
+                             is_valid_nonterminal ls nonterminal = true
+                             -> nonterminals_listT_R (remove_nonterminal ls nonterminal) ls;
+      ntl_wf : well_founded nonterminals_listT_R }.
+
+  Class parser_computational_types_dataT :=
+    { predata :> parser_computational_predataT;
+      split_stateT : String -> nonterminals_listT -> any_grammar CharType -> String -> Type }.
+
+  Class parser_computational_dataT' `{parser_computational_types_dataT} :=
+    { split_string_for_production
+      : forall (str0 : String) (valid : nonterminals_listT) (it : item CharType) (its : production CharType) (str : StringWithSplitState String (split_stateT str0 valid (it::its : production CharType))),
+          list (StringWithSplitState String (split_stateT str0 valid it)
+                * StringWithSplitState String (split_stateT str0 valid its));
+      split_string_for_production_correct
+      : forall str0 valid it its str,
+          let P f := List.Forall f (@split_string_for_production str0 valid it its str) in
+          P (fun s1s2 => (fst s1s2 ++ snd s1s2 =s str) = true) }.
+
+  Class parser_computational_dataT :=
+    { premethods :> parser_computational_types_dataT;
+      methods' :> parser_computational_dataT' }.
+
+  Class MonadT := Build_MonadT : Type -> Type.
+  Global Instance idM : MonadT | 10000 := fun x => x.
+  Global Strategy -1000 [idM].
+
+  Class parser_computational_prestrdataT `{parser_computational_dataT} `{M : MonadT} :=
+    { prelower_nonterminal_state
+      : forall {str0 valid nonterminal s},
+          split_stateT str0 valid (NonTerminal _ nonterminal) s -> M (split_stateT str0 valid (include_nonterminal _ nonterminal) s);
+
+      prelower_string_head
+      : forall {str0 valid}
+               {prod : production CharType}
+               {prods : productions CharType}
+               {s},
+          split_stateT str0 valid (prod::prods : productions CharType) s -> M (split_stateT str0 valid prod s);
+      prelower_string_tail
+      : forall {str0 valid}
+               {prod : production CharType}
+               {prods : productions CharType}
+               {s},
+          split_stateT str0 valid (prod::prods : productions CharType) s -> M (split_stateT str0 valid prods s);
+
+      prelift_lookup_nonterminal_state_lt
+      : forall {str0 valid nonterminal s} (pf : Length s < Length str0),
+          split_stateT str0 valid (include_nonterminal _ nonterminal) s -> M (split_stateT s initial_nonterminals_data (Lookup G nonterminal) s);
+
+      prelift_lookup_nonterminal_state_eq
+      : forall {str0 valid nonterminal s}
+               (pf : s = str0 :> String),
+          split_stateT str0 valid (include_nonterminal _ nonterminal) s -> M (split_stateT str0 (remove_nonterminal valid nonterminal) (Lookup G nonterminal) s) }.
+
+  Definition parser_computational_strdataT `{parser_computational_dataT} : Type
+    := parser_computational_prestrdataT.
+  Existing Class parser_computational_strdataT.
+
+  Definition lower_nonterminal_state `{methods : parser_computational_dataT, strdata : @parser_computational_strdataT methods}
+  : forall {str0 valid nonterminal s},
+      split_stateT _ _ _ _ -> split_stateT _ _ _ _
+    := @prelower_nonterminal_state methods (fun x => x) strdata.
+  Definition lower_string_head `{methods : parser_computational_dataT, strdata : @parser_computational_strdataT methods}
+  : forall {str0 valid prod prods s},
+      split_stateT _ _ _ _ -> split_stateT _ _ _ _
+    := @prelower_string_head methods (fun x => x) strdata.
+  Definition lower_string_tail `{methods : parser_computational_dataT, strdata : @parser_computational_strdataT methods}
+  : forall {str0 valid prod prods s},
+      split_stateT _ _ _ _ -> split_stateT _ _ _ _
+    := @prelower_string_tail methods (fun x => x) strdata.
+  Definition lift_lookup_nonterminal_state_lt `{methods : parser_computational_dataT, strdata : @parser_computational_strdataT methods}
+  : forall {str0 valid nonterminal s} pf,
+      split_stateT _ _ _ _ -> split_stateT _ _ _ _
+    := @prelift_lookup_nonterminal_state_lt methods (fun x => x) strdata.
+  Definition lift_lookup_nonterminal_state_eq `{methods : parser_computational_dataT, strdata : @parser_computational_strdataT methods}
+  : forall {str0 valid nonterminal s} pf,
+      split_stateT _ _ _ _ -> split_stateT _ _ _ _
+    := @prelift_lookup_nonterminal_state_eq methods (fun x => x) strdata.
+End recursive_descent_parser.
+
+Existing Class parser_computational_strdataT.
