src/Parsers/DependentlyTypedMinimalOfParseFactoredFull.v
@@ -1,6 +1,6 @@
 (** * Fully instantiated specialization of the dependently typed parser to minimal parse trees, taking in parse trees, using the factored abstraction barrier *)
 Require Import Coq.Lists.List Coq.Program.Program Coq.Program.Wf Coq.Arith.Wf_nat Coq.Arith.Compare_dec Coq.Classes.RelationClasses Coq.Strings.String.
-Require Import Parsers.ContextFreeGrammar Parsers.DependentlyTyped Parsers.MinimalParse.
+Require Import Parsers.ContextFreeGrammar Parsers.DependentlyTyped Parsers.MinimalParse Parsers.BaseTypes.
 Require Parsers.BooleanRecognizer Parsers.BooleanRecognizerCorrect.
 Require Import Parsers.DependentlyTypedMinimalOfParseFactored.
 Require Import Parsers.WellFoundedParse Parsers.ContextFreeGrammarProperties.
@@ -16,12 +16,12 @@ Section recursive_descent_parser.
   Context (G : grammar Ascii.ascii).
 
   Local Instance predata : parser_computational_predataT
-    := { nonterminal_names_listT := BooleanRecognizer.rdp_list_names_listT;
-         initial_nonterminal_names_data := Valid_nonterminal_symbols G;
-         is_valid_nonterminal_name := BooleanRecognizer.rdp_list_is_valid_name;
-         remove_nonterminal_name := BooleanRecognizer.rdp_list_remove_name;
-         nonterminal_names_listT_R := BooleanRecognizer.rdp_list_names_listT_R;
-         remove_nonterminal_name_dec := BooleanRecognizer.rdp_list_remove_name_dec;
+    := { nonterminals_listT := BooleanRecognizer.rdp_list_nonterminals_listT;
+         initial_nonterminals_data := Valid_nonterminals G;
+         is_valid_nonterminal := BooleanRecognizer.rdp_list_is_valid_nonterminal;
+         remove_nonterminal := BooleanRecognizer.rdp_list_remove_nonterminal;
+         nonterminals_listT_R := BooleanRecognizer.rdp_list_nonterminals_listT_R;
+         remove_nonterminal_dec := BooleanRecognizer.rdp_list_remove_nonterminal_dec;
          ntl_wf := BooleanRecognizer.rdp_list_ntl_wf }.
 
   Local Instance types_data : @parser_computational_types_dataT _ string_stringlike
@@ -37,7 +37,7 @@ Section recursive_descent_parser.
     intros; apply bool_eq_correct; assumption.
   Defined.
 
-  Local Instance strdata : @parser_computational_prestrdataT _ string_stringlike G {| DependentlyTyped.methods' := methods' |} idM.
+  Local Instance strdata : @parser_computational_prestrdataT _ string_stringlike G {| BaseTypes.methods' := methods' |} idM.
   Proof.
     constructor; simpl; intros; assumption.
   Defined.
@@ -46,7 +46,7 @@ Section recursive_descent_parser.
     := { methods' := methods' }.
 
   Lemma rdp_list_complete'
-        (str0 : string_stringlike) (valid : nonterminal_names_listT)
+        (str0 : string_stringlike) (valid : nonterminals_listT)
         (it : item Ascii.ascii) (its : production Ascii.ascii)
         (str : StringWithSplitState string_stringlike (split_stateT str0 valid (it :: its : production _)))
         (pf : str ≤s str0)
@@ -56,12 +56,7 @@ Section recursive_descent_parser.
     simpl.
     repeat intro.
     apply (@BooleanRecognizerCorrect.make_all_single_splits_complete
-             G BooleanRecognizer.rdp_list_names_listT
-             (Valid_nonterminal_symbols G)
-             BooleanRecognizer.rdp_list_is_valid_name
-             BooleanRecognizer.rdp_list_remove_name
-             {| string_val := str0 : string_stringlike ; state_val := I |}
-             valid valid
+             G str0 valid
              str
              pf (it::its : production _)).
     assumption.
@@ -72,22 +67,22 @@ Section recursive_descent_parser.
     := @minimal_of_parse_parser_dependent_types_extra_data'
          _ string_stringlike G
          predata methods' strdata
-         BooleanRecognizer.rdp_list_remove_name_1 BooleanRecognizer.rdp_list_remove_name_2
+         BooleanRecognizer.rdp_list_remove_nonterminal_1 BooleanRecognizer.rdp_list_remove_nonterminal_2
          rdp_list_complete'.
 
-  Definition minimal_parse_nonterminal_name__of__parse
-             (nonterminal_name : string)
+  Definition minimal_parse_nonterminal__of__parse
+             (nonterminal : string)
              (s : string)
-             (p : parse_of_item string_stringlike G s (NonTerminal _ nonterminal_name))
+             (p : parse_of_item string_stringlike G s (NonTerminal _ nonterminal))
              (H : Forall_parse_of_item
-                    (fun _ n => is_valid_nonterminal_name initial_nonterminal_names_data n = true)
+                    (fun _ n => is_valid_nonterminal initial_nonterminals_data n = true)
                     p)
-  : minimal_parse_of_name string_stringlike G initial_nonterminal_names_data is_valid_nonterminal_name remove_nonterminal_name s initial_nonterminal_names_data s nonterminal_name.
+  : minimal_parse_of_name string_stringlike G initial_nonterminals_data is_valid_nonterminal remove_nonterminal s initial_nonterminals_data s nonterminal.
   Proof.
-    eapply @minimal_parse_nonterminal_name__of__parse'.
+    eapply @minimal_parse_nonterminal__of__parse'.
     exact strdata.
-    exact BooleanRecognizer.rdp_list_remove_name_1.
-    exact BooleanRecognizer.rdp_list_remove_name_2.
+    exact BooleanRecognizer.rdp_list_remove_nonterminal_1.
+    exact BooleanRecognizer.rdp_list_remove_nonterminal_2.
     exact rdp_list_complete'.
     exact H.
   Defined.
