src/Parsers/DependentlyTypedSum.v
@@ -1,7 +1,7 @@
 (** * Specialization of the dependently typed parser to interleaving splitters *)
 Require Import Coq.Lists.List Coq.Program.Program Coq.Program.Wf Coq.Arith.Wf_nat Coq.Arith.Compare_dec Coq.Classes.RelationClasses Coq.Strings.String.
 Require Import Parsers.ContextFreeGrammar Parsers.DependentlyTyped.
-Require Import Parsers.WellFoundedParse Parsers.ContextFreeGrammarProperties.
+Require Import Parsers.WellFoundedParse Parsers.ContextFreeGrammarProperties Parsers.BaseTypes.
 Require Import Common Common.Wf Common.Le Common.Equality.
 
 Set Implicit Arguments.
@@ -37,14 +37,14 @@ Section recursive_descent_parser.
           strdata := leaf_strdata;
           extra_success_data := leaf_extra_success_data;
           extra_failure_data := leaf_extra_failure_data |}.
-  Context (remove_nonterminal_name_1
+  Context (remove_nonterminal_1
            : forall ls ps ps',
-               is_valid_nonterminal_name (remove_nonterminal_name ls ps) ps' = true
-               -> is_valid_nonterminal_name ls ps' = true)
-          (remove_nonterminal_name_2
+               is_valid_nonterminal (remove_nonterminal ls ps) ps' = true
+               -> is_valid_nonterminal ls ps' = true)
+          (remove_nonterminal_2
            : forall ls ps ps',
-               is_valid_nonterminal_name (remove_nonterminal_name ls ps) ps' = false
-               <-> is_valid_nonterminal_name ls ps' = false \/ ps = ps').
+               is_valid_nonterminal (remove_nonterminal ls ps) ps' = false
+               <-> is_valid_nonterminal ls ps' = false \/ ps = ps').
 
   Context top_split_stateT
           (top_methods' : @parser_computational_dataT' _ String {| split_stateT := top_split_stateT |}).
@@ -96,7 +96,7 @@ Section recursive_descent_parser.
   Proof. clear; abstract t_sum. Defined.
 
   Definition top_methods : @parser_computational_dataT _ String
-    := {| DependentlyTyped.methods' := top_methods' |}.
+    := {| BaseTypes.methods' := top_methods' |}.
 
   Variable top_prestrdata : @parser_computational_prestrdataT _ String G top_methods option.
 
@@ -114,16 +114,16 @@ Section recursive_descent_parser.
        end.
 
   Local Instance sum_prestrdata : @parser_computational_prestrdataT _ String G sum_methods idM
-    := { prelower_nonterminal_name_state str0 valid nonterminal_name str
-         := option_bind (@prelower_nonterminal_name_state _ _ _ _ _ top_prestrdata _ _ _ _);
+    := { prelower_nonterminal_state str0 valid nonterminal str
+         := option_bind (@prelower_nonterminal_state _ _ _ _ _ top_prestrdata _ _ _ _);
          prelower_string_head str0 valid prod prods str
          := option_bind (@prelower_string_head _ _ _ _ _ top_prestrdata _ _ _ _ _);
          prelower_string_tail str0 valid prod prods str
          := option_bind (@prelower_string_tail _ _ _ _ _ top_prestrdata _ _ _ _ _);
-         prelift_lookup_nonterminal_name_state_lt str0 valid nonterminal_name str pf
-         := option_bind (@prelift_lookup_nonterminal_name_state_lt _ _ _ _ _ top_prestrdata _ _ _ _ pf);
-         prelift_lookup_nonterminal_name_state_eq str0 valid nonterminal_name str pf
-         := option_bind (@prelift_lookup_nonterminal_name_state_eq _ _ _ _ _ top_prestrdata _ _ _ _ pf) }.
+         prelift_lookup_nonterminal_state_lt str0 valid nonterminal str pf
+         := option_bind (@prelift_lookup_nonterminal_state_lt _ _ _ _ _ top_prestrdata _ _ _ _ pf);
+         prelift_lookup_nonterminal_state_eq str0 valid nonterminal str pf
+         := option_bind (@prelift_lookup_nonterminal_state_eq _ _ _ _ _ top_prestrdata _ _ _ _ pf) }.
 
   Local Instance sum_strdata : @parser_computational_strdataT _ String G sum_methods := sum_prestrdata.
 
@@ -131,8 +131,8 @@ Section recursive_descent_parser.
   Local Notation etas str := (lift_StringWithSplitState str (fun _ => I)).
 
   Local Instance sum_stypes' : @parser_dependent_types_success_dataT' _ String sum_methods
-    := { T_nonterminal_name_success str0 valid name str
-         := @T_nonterminal_name_success _ _ _ leaf_stypes' str0 valid name (etas str);
+    := { T_nonterminal_success str0 valid name str
+         := @T_nonterminal_success _ _ _ leaf_stypes' str0 valid name (etas str);
          T_item_success str0 valid it str
          := @T_item_success _ _ _ leaf_stypes' str0 valid it (etas str);
          T_production_success str0 valid prod str
@@ -148,7 +148,7 @@ Section recursive_descent_parser.
   Local Instance sum_stypes : @parser_dependent_types_success_dataT _ String
     := {| stypes' := sum_stypes' |}.
   Local Instance sum_ftypes' : @parser_dependent_types_failure_dataT' _ String sum_stypes
-    := { T_nonterminal_name_failure := T_failureT (@T_nonterminal_name_failure);
+    := { T_nonterminal_failure := T_failureT (@T_nonterminal_failure);
          T_item_failure := T_failureT (@T_item_failure);
          T_production_failure := T_failureT (@T_production_failure);
          T_productions_failure := T_failureT (@T_productions_failure) }.
@@ -176,7 +176,7 @@ Section recursive_descent_parser.
 
   Global Instance sum_extra_success_data
   : @parser_dependent_types_extra_success_dataT' _ String G sum_stypes sum_strdata
-    := { lift_success str0 valid nonterminal_name str
+    := { lift_success str0 valid nonterminal str
          := liftA_str_I (@lift_success _ _ _ _ _ leaf_extra_success_data _ _ _ (etas str));
          parse_terminal_success str0 valid ch str
          := @parse_terminal_success _ _ _ _ _ leaf_extra_success_data _ _ _ (etas str);
@@ -188,10 +188,10 @@ Section recursive_descent_parser.
          := liftA_str_I (@lift_prods_success_head _ _ _ _ _ leaf_extra_success_data _ _ _ _ (etas str));
          lift_prods_success_tail str0 valid prod prods str
          := liftA_str_I (@lift_prods_success_tail _ _ _ _ _ leaf_extra_success_data _ _ _ _ (etas str));
-         lift_parse_nonterminal_name_success_lt str0 valid nonterminal_name str pf
-         := liftA_str_I (@lift_parse_nonterminal_name_success_lt _ _ _ _ _ leaf_extra_success_data _ _ _ (etas str) pf);
-         lift_parse_nonterminal_name_success_eq str0 valid nonterminal_name str pf H
-         := liftA_str_I (@lift_parse_nonterminal_name_success_eq _ _ _ _ _ leaf_extra_success_data _ _ _ (etas str) pf H) }.
+         lift_parse_nonterminal_success_lt str0 valid nonterminal str pf
+         := liftA_str_I (@lift_parse_nonterminal_success_lt _ _ _ _ _ leaf_extra_success_data _ _ _ (etas str) pf);
+         lift_parse_nonterminal_success_eq str0 valid nonterminal str pf H
+         := liftA_str_I (@lift_parse_nonterminal_success_eq _ _ _ _ _ leaf_extra_success_data _ _ _ (etas str) pf H) }.
 
   Local Obligation Tactic :=
     simpl;
@@ -207,13 +207,13 @@ Section recursive_descent_parser.
          lift_prods_failure_cross
          (H_prod_split_cross : forall str0 valid it its (str : StringWithSplitState String (top_split_stateT str0 valid (it :: its : production _))) (pf : str ≤s str0),
                                  @split_string_for_production _ _ _ top_methods' str0 valid it its (eta str) <> nil)
-         lift_parse_nonterminal_name_failure_lt_cross
-         lift_parse_nonterminal_name_failure_eq_cross
-         elim_parse_nonterminal_name_failure_cross
+         lift_parse_nonterminal_failure_lt_cross
+         lift_parse_nonterminal_failure_eq_cross
+         elim_parse_nonterminal_failure_cross
   : @parser_dependent_types_extra_failure_dataT' _ String G sum_types sum_strdata
-    := { lift_failure str0 valid nonterminal_name
+    := { lift_failure str0 valid nonterminal
          := option_rect_str
-              (fun str => impl_match_option _ (lift_failure_cross str0 valid nonterminal_name str))
+              (fun str => impl_match_option _ (lift_failure_cross str0 valid nonterminal str))
               (fun str => liftA_str_I (@lift_failure _ _ _ _ _ leaf_extra_failure_data _ _ _ (tts str)));
          parse_terminal_failure str0 valid ch
          := option_rect_str
@@ -238,18 +238,18 @@ Section recursive_descent_parser.
               (fun str pf => (@H_prod_split _ _ _ _ _ leaf_extra_failure_data _ _ _ _ (tts str) pf)
                                ∘ (fun H => eq_rect _ _ H _ _));
 
-         lift_parse_nonterminal_name_failure_lt str0 valid nonterminal_name
+         lift_parse_nonterminal_failure_lt str0 valid nonterminal
          := option_rect_str
-              (fun str pf => impl_match_option _ (lift_parse_nonterminal_name_failure_lt_cross str0 valid nonterminal_name str pf))
-              (fun str pf => liftA_str_I (@lift_parse_nonterminal_name_failure_lt _ _ _ _ _ leaf_extra_failure_data _ _ _ (tts str) pf));
-         lift_parse_nonterminal_name_failure_eq str0 valid nonterminal_name
+              (fun str pf => impl_match_option _ (lift_parse_nonterminal_failure_lt_cross str0 valid nonterminal str pf))
+              (fun str pf => liftA_str_I (@lift_parse_nonterminal_failure_lt _ _ _ _ _ leaf_extra_failure_data _ _ _ (tts str) pf));
+         lift_parse_nonterminal_failure_eq str0 valid nonterminal
          := option_rect_str
-              (fun str pf => impl_match_option _ (lift_parse_nonterminal_name_failure_eq_cross str0 valid nonterminal_name str pf))
-              (fun str pf => liftA_str_I (@lift_parse_nonterminal_name_failure_eq _ _ _ _ _ leaf_extra_failure_data _ _ _ (tts str) pf));
-         elim_parse_nonterminal_name_failure str0 valid nonterminal_name
+              (fun str pf => impl_match_option _ (lift_parse_nonterminal_failure_eq_cross str0 valid nonterminal str pf))
+              (fun str pf => liftA_str_I (@lift_parse_nonterminal_failure_eq _ _ _ _ _ leaf_extra_failure_data _ _ _ (tts str) pf));
+         elim_parse_nonterminal_failure str0 valid nonterminal
          := option_rect_str
-              (fun str => elim_parse_nonterminal_name_failure_cross str0 valid nonterminal_name str)
-              (fun str => @elim_parse_nonterminal_name_failure _ _ _ _ _ leaf_extra_failure_data _ _ _ (tts str)) }.
+              (fun str => elim_parse_nonterminal_failure_cross str0 valid nonterminal str)
+              (fun str => @elim_parse_nonterminal_failure _ _ _ _ _ leaf_extra_failure_data _ _ _ (tts str)) }.
   Next Obligation.
   Proof.
     intros.
@@ -283,9 +283,9 @@ Section recursive_descent_parser.
              fail_parse_nil_productions_cross
              lift_prods_failure_cross
              H_prod_split_cross
-             lift_parse_nonterminal_name_failure_lt_cross
-             lift_parse_nonterminal_name_failure_eq_cross
-             elim_parse_nonterminal_name_failure_cross
+             lift_parse_nonterminal_failure_lt_cross
+             lift_parse_nonterminal_failure_eq_cross
+             elim_parse_nonterminal_failure_cross
   : @parser_dependent_types_extra_dataT _ String G
     := {| DependentlyTyped.types := sum_types;
           DependentlyTyped.strdata := sum_strdata;
@@ -297,7 +297,7 @@ Section recursive_descent_parser.
                fail_parse_nil_productions_cross
                lift_prods_failure_cross
                H_prod_split_cross
-               lift_parse_nonterminal_name_failure_lt_cross
-               lift_parse_nonterminal_name_failure_eq_cross
-               elim_parse_nonterminal_name_failure_cross |}.
+               lift_parse_nonterminal_failure_lt_cross
+               lift_parse_nonterminal_failure_eq_cross
+               elim_parse_nonterminal_failure_cross |}.
 End recursive_descent_parser.
